WIP refactoring to separate modules

common/theories/LoopChecking/Common.v
@@ -15,3 +15,195 @@ Ltac rw_in l H := rewrite_strat (topdown l) in H.
 (* TODO move *)
 Arguments exist {A P}.
 Definition inspect {A} (x : A) : { y : A | x = y } := exist x eq_refl.
+
+Definition option_map2 {A} (f : A -> A -> A) (o o' : option A) : option A :=
+  match o, o' with
+  | Some x, Some y => Some (f x y)
+  | None, Some _
+  | Some _, None
+  | None, None => None
+  end.
+
+Derive Signature for InA.
+
+Lemma eqlistA_eq {A} (l l' : list A) : eqlistA Logic.eq l l' -> l = l'.
+Proof.
+  induction 1.
+  - reflexivity.
+  - now f_equal.
+Qed.
+
+#[export] Instance fold_left_ext {A B} : Proper (`=2` ==> eq ==> eq ==> eq) (@fold_left A B).
+Proof.
+  intros f g hfg ? ? -> ? ? ->.
+  induction y in y0 |- *; cbn; auto. now rewrite (hfg y0 a).
+Qed.
+
+(* None is smaller than anything *)
+Inductive opt_le {A} (le : relation A) : relation (option A) :=
+| opt_le_some x y : le x y -> opt_le le (Some x) (Some y)
+| opt_le_none_some x : opt_le le None x.
+Derive Signature for opt_le.
+
+Instance opt_le_refl {A} (le : relation A) : Reflexive le -> Reflexive (opt_le le).
+Proof.
+  intros hre x; induction x; constructor; reflexivity.
+Qed.
+
+Instance opt_le_trans {A} (le : relation A) : Transitive le -> Transitive (opt_le le).
+Proof.
+  intros hre x; induction x; destruct y as [y|]; intros z H H'; depelim H; depelim H'; constructor.
+  now transitivity y.
+Qed.
+
+
+Class Commutative {A} (f : A -> A -> A) := comm : forall x y, f x y = f y x.
+Instance option_map_2_comm {A} f : @Commutative A f -> @Commutative (option A) (option_map2 f).
+Proof.
+  intros com [x|] [y|] => //=. now rewrite comm.
+Qed.
+
+Instance Zmin_comm : Commutative Z.min := Z.min_comm.
+Instance Zmax_comm : Commutative Z.max := Z.max_comm.
+
+Instance nat_min_comm : Commutative Nat.min := Nat.min_comm.
+Instance nat_max_comm : Commutative Nat.max := Nat.max_comm.
+
+Class Associative {A} (f : A -> A -> A) := assoc : forall x y z, f x (f y z) = f (f x y) z.
+Instance option_map_2_assoc {A} f : @Associative A f -> @Associative (option A) (option_map2 f).
+Proof.
+  intros assoc [x|] [y|] [z|]; cbn => //. now rewrite assoc.
+Qed.
+
+Instance nat_min_assoc : Associative Nat.min := Nat.min_assoc.
+Instance nat_max_assoc : Associative Nat.max := Nat.max_assoc.
+
+
+Instance Zmin_assoc : Associative Z.min := Z.min_assoc.
+Instance Zmax_assoc : Associative Z.max := Z.max_assoc.
+
+Lemma fold_left_comm {A B} (f : B -> A -> B) (l : list A) (x : A) (acc : B) :
+  (forall x y z, f (f z x) y = f (f z y) x) ->
+  fold_left f l (f acc x) = f (fold_left f l acc) x.
+Proof.
+  intros.
+  induction l in acc, x |- *; cbn. auto.
+  rewrite -IHl. f_equal. now rewrite H.
+Qed.
+
+Lemma fold_left_min_opt_comm {A} (f : A -> A -> A) l x acc :
+  Associative f -> Commutative f ->
+  fold_left (option_map2 f) l (option_map2 f acc x) = option_map2 f (fold_left (option_map2 f) l acc) x.
+Proof.
+  intros ass c. rewrite fold_left_comm => //.
+  intros. rewrite -(assoc (f := option_map2 f)).
+  rewrite -(assoc (f := option_map2 f) z y x0).
+  f_equal. apply comm.
+Qed.
+
+Lemma fold_left_le {A B} {le} (f g : A -> B -> A) l :
+  (forall acc acc'  x, In x l -> le acc acc' -> le (f acc x) (g acc' x)) ->
+  forall acc acc', le acc acc' ->
+  le (fold_left f l acc) (fold_left g l acc').
+Proof.
+  intros hfg.
+  induction l => //. cbn. intros.
+  apply IHl. intros. apply hfg => //. now right. apply hfg => //. now left.
+Qed.
+
+Local Open Scope nat_scope.
+Lemma fold_left_ne_lt {A} (f g : nat -> A -> nat) l acc :
+  (forall x y z, f (f z x) y = f (f z y) x) ->
+  (forall x y z, g (g z x) y = g (g z y) x) ->
+  l <> [] ->
+  (forall acc acc' x, In x l -> (acc <= acc') -> (f acc x <= g acc' x)) ->
+  (forall acc acc' x, In x l -> (acc < acc') -> (f acc x < g acc' x)) ->
+  (exists x, In x l /\ forall acc acc', (acc <= acc') -> (f acc x < g acc' x)) ->
+  fold_left f l acc < fold_left g l acc.
+Proof.
+  intros hf hg.
+  generalize (Nat.le_refl acc).
+  generalize acc at 2 4.
+  induction l in acc |- * => //.
+  intros.
+  destruct l; cbn.
+  { destruct H3 as [x []]. cbn in H3. destruct H3; subst => //.
+    now eapply (H4 acc acc0). }
+  cbn in IHl.
+  rewrite hf hg.
+  rewrite fold_left_comm //. rewrite (fold_left_comm g) //.
+  destruct H3 as [min [hmin hfg]].
+  destruct hmin as [<-|hel].
+  - apply hfg. apply fold_left_le => //. intros; eapply H1 => //. now right; right.
+    apply H1 => //. now right; left.
+  - apply H2. now left. eapply IHl => //.
+    * intros acc1 acc' x hin. apply (H1 acc1 acc' x). now right.
+    * intros acc1 acc' x hin. apply (H2 acc1 acc' x). now right.
+    * exists min. split => //.
+Qed.
+Close Scope nat_scope.
+
+Notation min_opt := (option_map2 Z.min).
+
+Infix "≤" := (opt_le Z.le) (at level 50).
+
+Lemma opt_lt_le_trans x y z :
+  opt_le Z.lt x y ->
+  opt_le Z.le y z ->
+  opt_le Z.lt x z.
+Proof.
+  intros [] H'; depelim H'; constructor. lia.
+Qed.
+
+Lemma Zmin_opt_left x y : min_opt x y ≤ x.
+Proof.
+  destruct x as [x|], y as [y|]; constructor. lia.
+Qed.
+
+Lemma Zmin_opt_right x y : min_opt x y ≤ y.
+Proof.
+  destruct x as [x|], y as [y|]; constructor. lia.
+Qed.
+
+Lemma min_opt_spec x y z : min_opt x y = z -> (z = y \/ z = x).
+Proof.
+  destruct x as [x|], y as [y|], z as [z|]; cbn; intuition auto.
+  - noconf H. pose proof (Zmin_irreducible x y). destruct H; intuition (f_equal; auto).
+  - noconf H.
+Qed.
+
+Lemma fold_comm_assoc_nat x y z : option_map2 Nat.max x (option_map2 Nat.max y z) =
+  option_map2 Nat.max y (option_map2 Nat.max x z).
+Proof.
+  now rewrite (assoc (f := option_map2 Nat.max)) (comm (f := option_map2 Nat.max) x y) -assoc.
+Qed.
+
+Lemma fold_comm_assoc x y z : option_map2 Z.max x (option_map2 Z.max y z) =
+  option_map2 Z.max y (option_map2 Z.max x z).
+Proof.
+  now rewrite (assoc (f := option_map2 Z.max)) (comm (f := option_map2 Z.max) x y) -assoc.
+Qed.
+
+Notation max_opt := (option_map2 Z.max).
+
+Lemma max_opt_spec x y z : max_opt x y = Some z -> exists x' y', x = Some x' /\ y = Some y' /\ z = Z.max x' y'.
+Proof.
+  destruct x as [x|], y as [y|]; cbn; intuition eauto; try noconf H.
+  exists x, y. auto.
+Qed.
+
+#[export] Instance And3P_proper : Proper (iff ==> iff ==> iff ==> iff) ssrbool.and3.
+Proof.
+  repeat intro. split; intros []; split; intuition auto.
+Qed.
+
+#[export] Instance And4P_proper : Proper (iff ==> iff ==> iff ==> iff ==> iff) ssrbool.and4.
+Proof.
+  repeat intro. split; intros []; split; intuition auto.
+Qed.
+
+#[export] Instance And5P_proper : Proper (iff ==> iff ==> iff ==> iff ==> iff ==> iff) ssrbool.and5.
+Proof.
+  repeat intro. split; intros []; split; intuition auto.
+Qed.
+
