common/theories/LoopChecking/PartialLoopChecking.v
@@ -7,7 +7,7 @@ From MetaRocq.Utils Require Import utils.
 From MetaRocq.Common Require Universes.
 From Equations Require Import Equations.
 
-From MetaRocq.Common.LoopChecking Require Import Common Interfaces HornClauses.
+From MetaRocq.Common.LoopChecking Require Import Common Interfaces HornClauses Model.
 
 Set Equations Transparent.
 
@@ -41,1007 +41,16 @@ Module Type LoopCheckingItf (LS : LevelSets).
 End LoopCheckingItf.
 
 Module LoopCheckingImpl (LS : LevelSets).
-  Module Import Clauses := Clauses(LS).
+  Module Import Model := Model(LS).
 
   Local Open Scope Z_scope.
-
-Definition model := LevelMap.t (option Z).
-
-Definition level_value (m : model) (level : Level.t) : option Z :=
-  match LevelMap.find level m with
-  | Some v => v
-  | None => None
-  end.
-
-Definition levelexpr_value (m : model) (atom : LevelExpr.t) :=
-  level_value m (level atom).
-
-Extraction Inline levelexpr_value.
-
-Definition min_atom_value (m : model) (atom : LevelExpr.t) : option Z :=
-  let '(l, k) := atom in
-  match level_value m l with
-  | None => None
-  | Some val => Some (val - k)%Z
-  end.
-
-Definition option_map2 {A} (f : A -> A -> A) (o o' : option A) : option A :=
-  match o, o' with
-  | Some x, Some y => Some (f x y)
-  | None, Some _
-  | Some _, None
-  | None, None => None
-  end.
-
-Definition min_premise (m : model) (l : nonEmptyLevelExprSet) : option Z :=
-  let (hd, tl) := NonEmptySetFacts.to_nonempty_list l in
-  fold_left (fun min atom => option_map2 Z.min (min_atom_value m atom) min) tl (min_atom_value m hd).
-
-Definition satisfiable_atom (m : model) (atom : Level.t * Z) : bool :=
-  let '(l, k) := atom in
-  match level_value m l with
-  | Some val => k <=? val
-  | None => false
-  end.
-
-Definition satisfiable_premise (m : model) (l : nonEmptyLevelExprSet) :=
-  LevelExprSet.for_all (satisfiable_atom m) l.
-
-(* Definition valid_clause (m : model) (cl : clause) := *)
-  (* implb (satisfiable_premise m (premise cl)) (satisfiable_atom m (concl cl)). *)
-Definition level_value_above m l k :=
-  match level_value m l with
-  | Some val => k <=? val
-  | None => false
-  end.
-
-Definition valid_clause (m : model) (cl : clause) :=
-  let k0 := min_premise m (premise cl) in
-  match k0 with
-  | None => true
-  | Some k0 =>
-    let (l, k) := concl cl in
-    level_value_above m l (k + k0)
-  end.
-
-Definition is_model (cls : clauses) (m : model) : bool :=
-  Clauses.for_all (valid_clause m) cls.
-
-Inductive update_result :=
-  | VacuouslyTrue
-  | Holds
-  | DoesntHold (wm : LevelSet.t × model).
-
-Definition update_model (m : model) l v : model := LevelMap.add l (Some v) m.
-
-Definition update_value (m : model) (cl : clause) : option model :=
-  let k0 := min_premise m (premise cl) in
-  match k0 with
-  | None => None
-  | Some k0 =>
-    let (l, k) := concl cl in
-    (* Does the conclusion also hold?
-        We optimize a bit here, rather than adding k0 in a second stage,
-        we do it already while checking the clause. In the paper, a second
-        pass computes this.
-      *)
-    if level_value_above m l (k + k0) then None
-    else Some (update_model m l (k + k0))
-  end.
-
-Definition check_clause_model cl '(modified, m) :=
-    match update_value m cl with
-  | None => (modified, m)
-  | Some m => (clause_conclusion cl :: modified, m)
-  end.
-
-Definition check_model_aux (cls : clauses) (wm : list Level.t × model) : list Level.t × model :=
-  Clauses.fold check_clause_model cls wm.
-
-(* If check_model = None then we have a model of all clauses,
-  othewise, we return Some (W', m') where W ⊂ W' and the model has
-  been updated for at least one atom l ∈ W'. *)
-Definition check_model (cls : clauses) (wm : LevelSet.t × model) : option (LevelSet.t × model) :=
-  let '(modified, m) := check_model_aux cls ([], wm.2) in
-  match modified return option (LevelSet.t × model) with
-  | [] => None
-  | l => Some ((LevelSet.union (LevelSetProp.of_list l) wm.1), m)
-  end.
-
-Infix "=m" := LevelMap.Equal (at level 50).
-
-Definition strict_update m '(prems, (concl, k)) m' :=
-  exists v,
-  [/\ min_premise m prems = Some v, ~~ level_value_above m concl (k + v) &
-  m' =m (LevelMap.add concl (Some (k + v)) m)].
-
-Inductive strictly_updates cls : LevelSet.t -> model -> model -> Prop :=
-| update_one m cl m' : Clauses.In cl cls ->
-  strict_update m cl m' -> strictly_updates cls (LevelSet.singleton (clause_conclusion cl)) m m'
-| update_trans {ls ls' m m' m''} :
-  strictly_updates cls ls m m' ->
-  strictly_updates cls ls' m' m'' ->
-  strictly_updates cls (LevelSet.union ls ls') m m''.
-
-Lemma strictly_updates_step cls w m m' m'' :
-  strictly_updates cls w m m' ->
-  forall cl, Clauses.In cl cls -> strict_update m' cl m'' ->
-  strictly_updates cls (LevelSet.add (clause_conclusion cl) w) m m''.
-Proof.
-  induction 1.
-  - intros.
-    replace (LevelSet.add (clause_conclusion cl0) (LevelSet.singleton (clause_conclusion cl)))
-      with (LevelSet.union (LevelSet.singleton (clause_conclusion cl)) (LevelSet.singleton (clause_conclusion cl0))).
-    eapply update_trans; eapply update_one; tea.
-    eapply LevelSet.eq_leibniz. red. lsets.
-  - intros.
-    specialize (IHstrictly_updates2 _ H1 H2).
-    replace (LevelSet.add (clause_conclusion cl) (LevelSet.union ls ls'))
-      with (LevelSet.union ls (LevelSet.add (clause_conclusion cl) ls')).
-    eapply update_trans; tea.
-    eapply LevelSet.eq_leibniz. red. lsets.
-Qed.
-
-Lemma strictly_updates_weaken cls w cls' :
-  Clauses.Subset cls cls' ->
-  forall m m', strictly_updates cls w m m' -> strictly_updates cls' w m m'.
-Proof.
-  intros hcls m m'.
-  induction 1. constructor => //. now eapply hcls.
-  econstructor 2; tea.
-Qed.
-
-Lemma strictly_updates_W_trans cls m w m' cl m'' :
-  strictly_updates cls w m m' ->
-  strict_update m' cl m'' ->
-  strictly_updates (Clauses.add cl cls) (LevelSet.add (clause_conclusion cl) w) m m''.
-Proof.
-  intros updW su.
-  destruct cl as [prems [concl k]].
-  eapply strictly_updates_step; tea.
-  - eapply strictly_updates_weaken; tea. clsets.
-  - rewrite Clauses.add_spec. left; reflexivity.
-Qed.
-
-#[local] Instance Clauses_For_All_proper : Proper (eq ==> Clauses.Equal ==> iff) Clauses.For_all.
-Proof.
-  intros x y -> cl cl' eqcl.
-  unfold Clauses.For_all. now setoid_rewrite eqcl.
-Qed.
-
-#[local] Instance Clauses_for_all_proper : Proper (eq ==> Clauses.Equal ==> eq) Clauses.for_all.
-Proof.
-  intros x y -> cl cl' eqcl.
-  apply iff_is_true_eq_bool.
-  rewrite /is_true -!ClausesFact.for_all_iff. now rewrite eqcl.
-Qed.
-
-#[local] Instance is_model_proper : Proper (Clauses.Equal ==> eq ==> eq) is_model.
-Proof.
-  intros cl cl' eqcl x y ->. unfold is_model. now rewrite eqcl.
-Qed.
-
-
-Definition equal_model (m m' : model) := LevelMap.Equal m m'.
-
-#[local] Instance equal_model_equiv : Equivalence equal_model.
-Proof. unfold equal_model.
-  split; try econstructor; eauto.
-  red. intros. now symmetry.
-  red; intros. now transitivity y.
-Qed.
-
-
-#[local] Instance level_value_proper : Proper (equal_model ==> eq ==> eq) level_value.
-Proof.
-  intros x y eqm l ? <-. unfold level_value.
-  unfold equal_model in eqm.
-  destruct LevelMap.find eqn:hl.
-  - eapply LevelMap.find_2 in hl.
-    rewrite eqm in hl.
-    eapply LevelMap.find_1 in hl. now rewrite hl.
-  - eapply LevelMapFact.F.not_find_in_iff in hl.
-    rewrite eqm in hl.
-    eapply LevelMapFact.F.not_find_in_iff in hl.
-    now rewrite hl.
-Qed.
-
-#[local] Instance min_atom_value_proper : Proper (LevelMap.Equal ==> eq ==> eq) min_atom_value.
-Proof.
-  intros m m' eqm ? ? ->. unfold min_atom_value.
-  destruct y => //.
-  now rewrite eqm.
-Qed.
-
-#[local] Instance fold_left_ext {A B} : Proper (`=2` ==> eq ==> eq ==> eq) (@fold_left A B).
-Proof.
-  intros f g hfg ? ? -> ? ? ->.
-  induction y in y0 |- *; cbn; auto. now rewrite (hfg y0 a).
-Qed.
-
-#[local] Instance min_premise_proper : Proper (LevelMap.Equal ==> eq ==> eq) min_premise.
-Proof.
-  intros m m' eq ? ? ->.
-  unfold min_premise.
-  destruct to_nonempty_list.
-  now setoid_rewrite eq.
-Qed.
-
-#[local] Instance update_model_proper : Proper (LevelMap.Equal ==> eq ==> eq ==> LevelMap.Equal) update_model.
-Proof.
-  intros m m' hm ? ? -> ? ? ->.
-  unfold update_model.
-  now rewrite hm.
-Qed.
-
-#[local] Instance level_value_above_proper : Proper (LevelMap.Equal ==> eq ==> eq ==> eq) level_value_above.
-Proof.
-  intros m m' hm ? ? -> ? ? ->.
-  unfold level_value_above.
-  now rewrite hm.
-Qed.
-
-Lemma eqlistA_eq {A} (l l' : list A) : eqlistA Logic.eq l l' -> l = l'.
-Proof.
-  induction 1.
-  - reflexivity.
-  - now f_equal.
-Qed.
-
-Instance clauses_elements_proper : Proper (Clauses.Equal ==> eq) Clauses.elements.
-Proof.
-  intros cl cl' eq.
-  have sl := Clauses.elements_spec2 cl.
-  (* have nl := Clauses.elements_spec2w cl. *)
-  have sl' := Clauses.elements_spec2 cl'.
-  (* have nl' := Clauses.elements_spec2w cl'. *)
-  have heq := @SortA_equivlistA_eqlistA _ Logic.eq _ Clause.lt_.
-  do 3 forward heq by tc.
-  specialize (heq _ _ sl sl').
-  forward heq.
-  red. intros x.
-  rewrite -! ClausesProp.Dec.F.elements_iff. apply eq.
-  now apply eqlistA_eq.
-Qed.
-
-#[local] Instance check_model_aux_proper : Proper (Clauses.Equal ==> eq ==> eq) check_model_aux.
-Proof.
-  intros ? ? eq ? ? ->.
-  rewrite /check_model_aux.
-  rewrite !ClausesProp.fold_spec_right.
-  now rewrite eq.
-Qed.
-
-#[local] Instance check_model_proper : Proper (Clauses.Equal ==> eq ==> eq) check_model.
-Proof.
-  intros cls cls' eq.
-  intros wm wm' ->.
-  unfold check_model.
-  destruct (check_model_aux cls _) eqn:eqc.
-  destruct (check_model_aux cls' _) eqn:eqc' => //.
-  pose proof (check_model_aux_proper cls cls' eq ([], wm'.2) _ eq_refl).
-  rewrite eqc eqc' in H. noconf H.
-  destruct l => //.
-Qed.
-
-Instance strictly_updates_proper : Proper (Clauses.Equal ==> LevelSet.Equal ==> LevelMap.Equal ==> LevelMap.Equal ==> iff) strictly_updates.
-Proof.
-  intros ? ? H ? ? H' ? ? H'' ? ? H'''.
-  eapply LevelSet.eq_leibniz in H'. subst y0.
-  split.
-  induction 1 in y, H, y1, H'', y2, H'''|- * ; [econstructor 1|econstructor 2]; eauto.
-  now rewrite <- H. move: H1; unfold strict_update. destruct cl as [premse []].
-  intros [v []]; exists v; split;
-  try setoid_rewrite <- H;
-  try setoid_rewrite <- H'';
-  try setoid_rewrite <- H'''; firstorder.
-  eapply IHstrictly_updates1; firstorder. firstorder.
-  induction 1 in x, H, x1, H'', x2, H'''|- * ; [econstructor 1|econstructor 2]; eauto.
-  now rewrite H. move: H1; unfold strict_update. destruct cl as [premse []].
-  intros [v []]; exists v; split;
-  try setoid_rewrite H;
-  try setoid_rewrite H'';
-  try setoid_rewrite H'''; firstorder.
-  eapply IHstrictly_updates1; firstorder. firstorder.
-Qed.
-
-Lemma update_value_valid {m cl} :
-  match update_value m cl with
-  | None => valid_clause m cl
-  | Some _ => ~~ valid_clause m cl
-  end.
-Proof.
-  unfold update_value, valid_clause.
-  destruct cl as [prem [l k]]; cbn.
-  destruct min_premise => //.
-  unfold level_value_above;
-  destruct level_value => //.
-  destruct Z.leb => //.
-Qed.
-
-Lemma check_clause_model_spec {cl w m w' m'} :
-  check_clause_model cl (w, m) = (w', m') ->
-  (w = w' -> m = m' /\ valid_clause m cl) /\
-  (w <> w' -> w' = clause_conclusion cl :: w /\
-    strictly_updates (Clauses.singleton cl) (LevelSet.singleton (clause_conclusion cl)) m m').
-Proof.
-  unfold check_clause_model.
-  destruct update_value eqn:upd; revgoals.
-  * intros [= <- <-]. split => //. split => //.
-    move: (@update_value_valid m cl). now rewrite upd.
-  * intros [= <- <-]. split => //.
-    + intros. eapply (f_equal (@List.length _)) in H. cbn in H; lia.
-    + intros _. split => //. constructor. clsets. unfold strict_update.
-      move: upd. unfold update_value.
-      destruct cl as [prems [concl k]]. cbn.
-      destruct min_premise => //.
-      destruct level_value_above eqn:hl => //.
-      intros [= <-].
-      exists z. split => //. rewrite hl. split => //.
-Qed.
-
-Derive Signature for InA.
-
-Lemma check_model_aux_spec {cls w m w' m'} :
-  check_model_aux cls (w, m) = (w', m') ->
-  (w = w' -> m = m' /\ is_model cls m) /\
-  (w <> w' -> exists pref, w' = pref ++ w /\ strictly_updates cls (LevelSetProp.of_list pref) m m').
-Proof.
-  rewrite /check_model_aux /is_model.
-  revert w' m'.
-  eapply ClausesProp.fold_rec.
-  - intros s' he w' m' [= <- <-]. split => //. split => //.
-    eapply Clauses.for_all_spec. tc. intros x hin. now apply he in hin.
-  - clear. intros x [w'' m''] s' s'' inx nins' hadd ih w' m' cl.
-    specialize (ih _ _ eq_refl) as[].
-    split; intros; subst.
-    + eapply check_clause_model_spec in cl as [].
-      destruct (eqb_spec w' w'').
-      { subst w''. specialize (H eq_refl) as []. specialize (H1 eq_refl) as []. split => //. congruence.
-        eapply Clauses.for_all_spec in H3. eapply Clauses.for_all_spec. all:tc.
-        intros ? hin. eapply hadd in hin as []; subst; firstorder. }
-      forward H0 by auto. forward H2 by auto.
-      destruct H0 as [pref [-> su]].
-      destruct pref; cbn in *; try congruence.
-      destruct H2. eapply (f_equal (@List.length _)) in H0; cbn in H0. rewrite length_app in H0. lia.
-    + eapply check_clause_model_spec in cl as [].
-      destruct (eqb_spec w w'').
-      { subst w''. specialize (H eq_refl) as []. subst m''.
-        destruct (eqb_spec w w'); subst; try congruence.
-        specialize (H3 H) as []. subst w'. exists [clause_conclusion x]. split => //.
-        replace (LevelSetProp.of_list [clause_conclusion x]) with (LevelSet.singleton (clause_conclusion x)).
-        eapply ClausesProp.Add_Equal in hadd. rewrite hadd. eapply strictly_updates_weaken; tea. clsets.
-        eapply LevelSet.eq_leibniz. red. intros ?. rewrite LevelSetProp.of_list_1. firstorder. constructor.
-        rewrite LevelSet.singleton_spec in H3. firstorder. depelim H3. subst. lsets. depelim H3. }
-      specialize (H0 H4).
-      destruct (eqb_spec w'' w'); subst.
-      { specialize (H2 eq_refl) as []; subst m''.
-        destruct H0 as [pref []]. subst w'. exists pref; split => //.
-        eapply strictly_updates_weaken; tea. intros ? ?. eapply hadd. clsets. }
-      forward H3 by auto. destruct H3 as [->].
-      destruct H0 as [pref [-> su]]. eexists (clause_conclusion x :: pref); split => //.
-      replace (LevelSetProp.of_list (clause_conclusion x :: pref)) with (LevelSet.union (LevelSetProp.of_list pref) (LevelSet.singleton (clause_conclusion x))).
-      eapply (strictly_updates_weaken _ _ s'') in su; tea; try firstorder.
-      eapply (strictly_updates_weaken _ _ s'') in H3; tea; try firstorder.
-      2:{ intros ?; rewrite Clauses.singleton_spec. intros ->. now apply hadd. }
-      exact: update_trans _ su H3.
-      apply LevelSet.eq_leibniz. intros ?. cbn. lsets.
-Qed.
-
-Lemma check_model_spec {cls w m w' m'} :
-  check_model cls (w, m) = Some (w', m') ->
-  exists w'', strictly_updates cls w'' m m' /\ w' = LevelSet.union w w''.
-Proof.
-  unfold check_model.
-  destruct check_model_aux eqn:cm.
-  apply check_model_aux_spec in cm as [].
-  destruct l => //. forward H0. auto with datatypes.
-  intros [= <- <-]. destruct H0 as [pref [heq su]].
-  rewrite app_nil_r in heq. subst pref.
-  exists (LevelSetProp.of_list (t :: l)). split => //.
-  eapply LevelSet.eq_leibniz. intros ?. cbn. lsets.
-Qed.
-
-
-Lemma strict_update_invalid m cl m' : strict_update m cl m' -> ~~ valid_clause m cl.
-Proof.
-  destruct cl as [prems [concl k]].
-  cbn.
-  intros [v [him hna heq]].
-  rewrite /valid_clause. rewrite him //=.
-Qed.
-
-Lemma strictly_updates_invalid cls w m m' : strictly_updates cls w m m' -> ~~ is_model cls m.
-Proof.
-  induction 1.
-  - eapply strict_update_invalid in H0.
-    apply/negbT. unfold is_model.
-    destruct Clauses.for_all eqn:fa => //.
-    eapply Clauses.for_all_spec in fa; tc. eapply fa in H.
-    now rewrite H in H0.
-  - auto.
-Qed.
-
-Lemma check_model_None {cls acc} :
-  check_model cls acc = None <-> is_model cls acc.2.
-Proof.
-  unfold check_model.
-  destruct check_model_aux eqn:cm.
-  apply check_model_aux_spec in cm as [ne ex].
-  destruct l => //. split => // _. now specialize (ne eq_refl) as [].
-  split => //. forward ex by auto with datatypes. destruct ex as [pref [eq su]].
-  rewrite app_nil_r in eq; subst pref.
-  intros ism. eapply strictly_updates_invalid in su.
-  now rewrite ism in su.
-Qed.
-
-Lemma check_model_updates_spec {cls w init_model m w' m'} :
-  check_model cls (w, m) = Some (w', m') ->
-  forall cls', strictly_updates cls' w init_model m ->
-  strictly_updates (Clauses.union cls cls') w' init_model m' /\ w ⊂_lset w'.
-Proof.
-  move/check_model_spec => [w'' [su ->]].
-  intros cls' su'. split.
-  eapply update_trans; eapply strictly_updates_weaken; tea; clsets. lsets.
-Qed.
-
-Lemma strictly_updates_non_empty {cls W m m'} :
-  strictly_updates cls W m m' -> ~ LevelSet.Empty W.
-Proof.
-  induction 1.
-  - intros he. specialize (he (clause_conclusion cl)). lsets.
-  - intros he. apply IHstrictly_updates2. lsets.
-Qed.
-
-Lemma strictly_updates_non_empty_map {cls W m m'} :
-  strictly_updates cls W m m' -> ~ LevelMap.Empty m'.
-Proof.
-  induction 1.
-  - intros he. specialize (he (clause_conclusion cl)).
-    destruct cl as [prems [concl k]].
-    destruct H0 as [? [? ? heq]].
-    setoid_rewrite heq in he. eapply (he (Some (k + x))); cbn.
-    rewrite LevelMapFact.F.add_mapsto_iff. firstorder.
-  - intros he. now apply IHstrictly_updates2.
-Qed.
-
-Definition clauses_conclusions (cls : clauses) : LevelSet.t :=
-  Clauses.fold (fun cl acc => LevelSet.add (level (concl cl)) acc) cls LevelSet.empty.
-
-Lemma clauses_conclusions_spec a cls :
-  LevelSet.In a (clauses_conclusions cls) <->
-  exists cl, Clauses.In cl cls /\ level (concl cl) = a.
-Proof.
-  unfold clauses_conclusions.
-  eapply ClausesProp.fold_rec; clear.
-  - move=> s' he /=. rewrite LevelSetFact.empty_iff.
-    firstorder auto.
-  - move=> cl ls cls' cls'' hin hnin hadd ih.
-    rewrite LevelSet.add_spec. firstorder eauto.
-    specialize (H0 x). cbn in H0.
-    apply hadd in H1. firstorder eauto.
-    subst. left. now destruct x.
-Qed.
-
-Lemma strictly_updates_incl {cls W m m'} :
-  strictly_updates cls W m m' -> W ⊂_lset clauses_conclusions cls.
-Proof.
-  induction 1.
-  - intros x. rewrite clauses_conclusions_spec. firstorder. exists cl.
-    eapply LevelSet.singleton_spec in H1; red in H1; subst. split => //.
-  - lsets.
-Qed.
-
-Lemma check_model_subset {cls v} :
-  forall w' v', check_model cls v = Some (w', v') -> ~ LevelSet.Empty w'.
-Proof.
-  intros w' v'.
-  move/check_model_spec => [w'' [su ->]].
-  eapply strictly_updates_non_empty in su. intros em. apply su. lsets.
-Qed.
-
-Definition premise_restricted_to W cl :=
-  LevelSet.subset (levels (premise cl)) W.
-
-Definition clause_restricted_to W cl :=
-  LevelSet.subset (levels (premise cl)) W &&
-  LevelSet.mem (level (concl cl)) W.
-
-Definition restrict_clauses (cls : clauses) (W : LevelSet.t) :=
-  Clauses.filter (clause_restricted_to W) cls.
-
-Lemma in_restrict_clauses (cls : clauses) (concls : LevelSet.t) cl :
-  Clauses.In cl (restrict_clauses cls concls) <->
-  [/\ LevelSet.In (level (concl cl)) concls,
-    LevelSet.Subset (levels (premise cl)) concls &
-    Clauses.In cl cls].
-Proof.
-  unfold restrict_clauses.
-  rewrite Clauses.filter_spec.
-  destruct cl. cbn.
-  rewrite andb_true_iff LevelSet.subset_spec LevelSet.mem_spec.
-  firstorder auto.
-Qed.
-
-Lemma restrict_clauses_subset (cls : clauses) (concls : LevelSet.t) : Clauses.Subset (restrict_clauses cls concls) cls.
-Proof.
-  intros x; rewrite in_restrict_clauses; now intros [].
-Qed.
-
-Definition clauses_with_concl (cls : clauses) (concl : LevelSet.t) :=
-  Clauses.filter (fun '(prem, concla) => LevelSet.mem (level concla) concl) cls.
-
-Lemma in_clauses_with_concl (cls : clauses) (concls : LevelSet.t) cl :
-  Clauses.In cl (clauses_with_concl cls concls) <->
-  LevelSet.In (level (concl cl)) concls /\ Clauses.In cl cls.
-Proof.
-  unfold clauses_with_concl.
-  rewrite Clauses.filter_spec.
-  destruct cl. rewrite LevelSet.mem_spec. cbn. firstorder eauto.
-Qed.
-
-Lemma clauses_conclusions_clauses_with_concl cls concl :
-  LevelSet.Subset (clauses_conclusions (clauses_with_concl cls concl)) concl.
-Proof.
-  intros x [cl []] % clauses_conclusions_spec.
-  eapply in_clauses_with_concl in H as [].
-  now rewrite H0 in H.
-Qed.
-
-Lemma clauses_conclusions_restrict_clauses cls W :
-  LevelSet.Subset (clauses_conclusions (restrict_clauses cls W)) W.
-Proof.
-  intros x [cl []] % clauses_conclusions_spec.
-  eapply in_restrict_clauses in H as [].
-  now rewrite H0 in H.
-Qed.
-
-Definition in_clauses_conclusions (cls : clauses) (x : Level.t): Prop :=
-  exists cl, Clauses.In cl cls /\ (level cl.2) = x.
-
 Definition v_minus_w_bound (W : LevelSet.t) (m : model) :=
   LevelMap.fold (fun w v acc => Z.max (option_get 0 v) acc)
     (LevelMapFact.filter (fun l _ => ~~ LevelSet.mem l W) m) 0%Z.
 
-Definition premise_min (l : nonEmptyLevelExprSet) : Z :=
-  let (hd, tl) := NonEmptySetFacts.to_nonempty_list l in
-  fold_left (B:=LevelExpr.t) (fun min atom => Z.min atom.2 min) tl (hd.2).
-
-Definition premise_max (l : nonEmptyLevelExprSet) : Z :=
-  let (hd, tl) := NonEmptySetFacts.to_nonempty_list l in
-  fold_left (B:=LevelExpr.t) (fun min atom => Z.max atom.2 min) tl (hd.2).
-
-Definition gain (cl : clause) : Z :=
-  (concl cl).2 - (premise_min (premise cl)).
-
-Definition max_gain (cls : clauses) :=
-  Clauses.fold (fun cl acc => Nat.max (Z.to_nat (gain cl)) acc) cls 0%nat.
-
-Definition max_clause_premise (cls : clauses) :=
-  Clauses.fold (fun cl acc => Z.max (premise_max (premise cl)) acc) cls 0%Z.
-
-Definition model_same_domain (m m' : model) :=
-  forall l, LevelMap.In l m <-> LevelMap.In l m'.
-
-#[local] Instance model_same_domain_refl : Reflexive model_same_domain.
-Proof. intros m l. reflexivity. Qed.
-
-#[local] Instance model_same_domain_trans : Transitive model_same_domain.
-Proof. intros m m' m'' h h' l. rewrite (h l). apply h'. Qed.
-
-
-Inductive opt_le {A} (le : relation A) : relation (option A) :=
-| opt_le_some x y : le x y -> opt_le le (Some x) (Some y)
-| opt_le_none_some x : opt_le le None x.
-Derive Signature for opt_le.
-
-Instance opt_le_refl {A} (le : relation A) : Reflexive le -> Reflexive (opt_le le).
-Proof.
-  intros hre x; induction x; constructor; reflexivity.
-Qed.
-
-Instance opt_le_trans {A} (le : relation A) : Transitive le -> Transitive (opt_le le).
-Proof.
-  intros hre x; induction x; destruct y as [y|]; intros z H H'; depelim H; depelim H'; constructor.
-  now transitivity y.
-Qed.
-
-Infix "≤" := (opt_le Z.le) (at level 50).
-
-Infix "≤Z" := (opt_le Z.le) (at level 50).
-
-Definition model_rel R (m m' : model) :=
-  forall l k, LevelMap.MapsTo l k m -> exists k', LevelMap.MapsTo l k' m' /\ R k k'.
-
-Infix "⩽" := (model_rel (opt_le Z.le)) (at level 70). (* \leqslant *)
-
-Definition model_map_outside V (m m' : model) :=
-  forall l, ~ LevelSet.In l V ->
-    forall k, LevelMap.MapsTo l k m <-> LevelMap.MapsTo l k m'.
-
-#[local] Instance model_map_outside_refl V : Reflexive (model_map_outside V).
-Proof. intros m l. reflexivity. Qed.
-
-#[local] Instance model_map_outside_trans V : Transitive (model_map_outside V).
-Proof.
-  intros m m' m'' h h' l hnin k.
-  rewrite (h l hnin k). now apply h'.
-Qed.
-
 (** The termination proof relies on the correctness of check_model:
   it does strictly increase a value but not above [max_gain cls].
 *)
-
-Lemma clauses_conclusions_diff cls s :
-  clauses_conclusions (Clauses.diff cls (clauses_with_concl cls s)) ⊂_lset
-  LevelSet.diff (clauses_conclusions cls) s.
-Proof.
-  intros a. rewrite LevelSet.diff_spec !clauses_conclusions_spec.
-  firstorder eauto.
-  exists x; split => //.
-  now rewrite Clauses.diff_spec in H.
-  intros ha.
-  rewrite Clauses.diff_spec in H; destruct H as [].
-  apply H1.
-  rewrite in_clauses_with_concl. split => //.
-  now rewrite H0.
-Qed.
-
-Lemma diff_eq U V : LevelSet.diff V U =_lset V <-> LevelSet.inter V U =_lset LevelSet.empty.
-Proof. split. lsets. lsets. Qed.
-
-Lemma levelset_neq U V : LevelSet.equal U V = false -> ~ LevelSet.Equal U V.
-Proof. intros eq heq % LevelSet.equal_spec. congruence. Qed.
-
-Lemma levelset_union_same U : LevelSet.union U U =_lset U.
-Proof. lsets. Qed.
-
-Class Commutative {A} (f : A -> A -> A) := comm : forall x y, f x y = f y x.
-Instance option_map_2_comm {A} f : @Commutative A f -> @Commutative (option A) (option_map2 f).
-Proof.
-  intros com [x|] [y|] => //=. now rewrite comm.
-Qed.
-
-Instance Zmin_comm : Commutative Z.min := Z.min_comm.
-Instance Zmax_comm : Commutative Z.max := Z.max_comm.
-
-Instance nat_min_comm : Commutative Nat.min := Nat.min_comm.
-Instance nat_max_comm : Commutative Nat.max := Nat.max_comm.
-
-Class Associative {A} (f : A -> A -> A) := assoc : forall x y z, f x (f y z) = f (f x y) z.
-Instance option_map_2_assoc {A} f : @Associative A f -> @Associative (option A) (option_map2 f).
-Proof.
-  intros assoc [x|] [y|] [z|]; cbn => //. now rewrite assoc.
-Qed.
-
-Instance nat_min_assoc : Associative Nat.min := Nat.min_assoc.
-Instance nat_max_assoc : Associative Nat.max := Nat.max_assoc.
-
-
-Instance Zmin_assoc : Associative Z.min := Z.min_assoc.
-Instance Zmax_assoc : Associative Z.max := Z.max_assoc.
-
-Lemma fold_left_comm {A B} (f : B -> A -> B) (l : list A) (x : A) (acc : B) :
-  (forall x y z, f (f z x) y = f (f z y) x) ->
-  fold_left f l (f acc x) = f (fold_left f l acc) x.
-Proof.
-  intros.
-  induction l in acc, x |- *; cbn. auto.
-  rewrite -IHl. f_equal. now rewrite H.
-Qed.
-
-Lemma fold_left_min_opt_comm {A} (f : A -> A -> A) l x acc :
-  Associative f -> Commutative f ->
-  fold_left (option_map2 f) l (option_map2 f acc x) = option_map2 f (fold_left (option_map2 f) l acc) x.
-Proof.
-  intros ass c. rewrite fold_left_comm => //.
-  intros. rewrite -(assoc (f := option_map2 f)).
-  rewrite -(assoc (f := option_map2 f) z y x0).
-  f_equal. apply comm.
-Qed.
-
-Lemma fold_left_le {A} {le} (f g : A -> LevelSet.elt -> A) l :
-  (forall acc acc'  x, In x l -> le acc acc' -> le (f acc x) (g acc' x)) ->
-  forall acc acc', le acc acc' ->
-  le (fold_left f l acc) (fold_left g l acc').
-Proof.
-  intros hfg.
-  induction l => //. cbn. intros.
-  apply IHl. intros. apply hfg => //. now right. apply hfg => //. now left.
-Qed.
-
-Local Open Scope nat_scope.
-Lemma fold_left_ne_lt (f g : nat -> LevelSet.elt -> nat) l acc :
-  (forall (x y : LevelSet.elt) z, f (f z x) y = f (f z y) x) ->
-  (forall (x y : LevelSet.elt) z, g (g z x) y = g (g z y) x) ->
-  l <> [] ->
-  (forall acc acc' x, In x l -> (acc <= acc') -> (f acc x <= g acc' x)) ->
-  (forall acc acc' x, In x l -> (acc < acc') -> (f acc x < g acc' x)) ->
-  (exists x, In x l /\ forall acc acc', (acc <= acc') -> (f acc x < g acc' x)) ->
-  fold_left f l acc < fold_left g l acc.
-Proof.
-  intros hf hg.
-  generalize (Nat.le_refl acc).
-  generalize acc at 2 4.
-  induction l in acc |- * => //.
-  intros.
-  destruct l; cbn.
-  { destruct H3 as [x []]. cbn in H3. destruct H3; subst => //.
-    now eapply (H4 acc acc0). }
-  cbn in IHl.
-  rewrite hf hg.
-  rewrite fold_left_comm //. rewrite (fold_left_comm g) //.
-  destruct H3 as [min [hmin hfg]].
-  destruct hmin as [<-|hel].
-  - apply hfg. apply fold_left_le => //. intros; eapply H1 => //. now right; right.
-    apply H1 => //. now right; left.
-  - apply H2. now left. eapply IHl => //.
-    * intros acc1 acc' x hin. apply (H1 acc1 acc' x). now right.
-    * intros acc1 acc' x hin. apply (H2 acc1 acc' x). now right.
-    * exists min. split => //.
-Qed.
-Close Scope nat_scope.
-
-Infix "↓" := clauses_with_concl (at level 70). (* \downarrow *)
-Infix "⇂" := restrict_clauses (at level 70). (* \downharpoonright *)
-
-Lemma clauses_conclusions_diff_left cls W cls' :
-  clauses_conclusions (Clauses.diff (cls ↓ W) cls') ⊂_lset W.
-Proof.
-  intros l.
-  rewrite clauses_conclusions_spec.
-  move=> [] cl. rewrite Clauses.diff_spec => [] [] [].
-  move/in_clauses_with_concl => [] hin ? ? eq.
-  now rewrite eq in hin.
-Qed.
-
-Lemma clauses_conclusions_diff_restrict cls W cls' :
-  clauses_conclusions (Clauses.diff (cls ⇂ W) cls') ⊂_lset W.
-Proof.
-  intros l.
-  rewrite clauses_conclusions_spec.
-  move=> [] cl. rewrite Clauses.diff_spec => [] [] [].
-  move/in_restrict_clauses => [] hin ? ? ? eq.
-  now rewrite eq in hin.
-Qed.
-
-Lemma LevelSet_In_elements l s :
-  In l (LevelSet.elements s) <-> LevelSet.In l s.
-Proof.
-  rewrite LevelSetFact.elements_iff.
-  now rewrite InA_In_eq.
-Qed.
-
-Lemma clauses_empty_eq {s} : Clauses.Empty s -> Clauses.Equal s Clauses.empty.
-Proof. clsets. Qed.
-
-Lemma valid_update_value {m cl} :
-  valid_clause m cl ->
-  match update_value m cl with
-  | None => true
-  | Some _ => false
-  end.
-Proof.
-  unfold update_value, valid_clause.
-  destruct cl as [prem [l k]]; cbn.
-  destruct min_premise => //.
-  unfold level_value_above.
-  destruct level_value => //.
-  destruct Z.leb => //.
-Qed.
-
-Lemma level_value_not_above_spec m l k : level_value_above m l k = false -> opt_le Z.lt (level_value m l) (Some k).
-Proof.
-  unfold level_value_above; destruct level_value => // hlt; constructor. lia.
-Qed.
-
-Lemma clauses_for_all_neg {p s}:
-  ~~ Clauses.for_all p s <-> ~ Clauses.For_all p s.
-Proof.
-  intuition auto.
-  rewrite ClausesFact.for_all_iff in H0. red in H. now rewrite H0 in H.
-  revert H. apply contra_notN.
-  rewrite ClausesFact.for_all_iff //.
-Qed.
-
-Lemma clauses_for_all_exists {p s}:
-  ~~ Clauses.for_all p s <-> Clauses.exists_ (fun x => ~~ p x) s.
-Proof.
-  rewrite ClausesFact.for_all_b ClausesFact.exists_b.
-  induction (Clauses.elements s).
-  - cbn; auto. reflexivity.
-  - cbn. rewrite negb_and. intuition auto.
-    move/orP: H1 => [->|] //. move/H. intros ->. now rewrite orb_true_r.
-    move/orP: H1 => [->|] //. move/H0. intros ->. now rewrite orb_true_r.
-Qed.
-#[local] Instance model_le_refl R (HR : Reflexive R) : Reflexive (model_rel R).
-Proof. intros x l k map. exists k; split => //. Qed.
-
-#[local] Instance model_le_trans R (HR : Transitive R) : Transitive (model_rel R).
-Proof. intros m m' m'' mm' m'm'' l k map.
-  apply mm' in map as [k' [map ?]].
-  apply m'm'' in map as [k'' [map ?]]. exists k''. split => //.
-  now transitivity k'.
-Qed.
-
-Lemma update_model_monotone m l k : level_value m l ≤ Some k ->
-  m ⩽ update_model m l k.
-Proof.
-  intros hl.
-  intros l' k' maps.
-  unfold update_model. cbn.
-  destruct (eqb_spec l l').
-  - subst l'. exists (Some k). move: hl.
-    unfold level_value.
-    rewrite (LevelMap.find_1 maps).
-    intros hle.
-    split => //. eapply LevelMap.add_1. eapply LevelMap.OT.eq_refl.
-  - exists k'. split => //. apply LevelMap.add_2 => //. reflexivity.
-Qed.
-
-Lemma update_model_not_above m l k : level_value_above m l k = false ->
-  m ⩽ update_model m l k.
-Proof.
-  unfold level_value_above.
-  intros hlev.
-  apply update_model_monotone.
-  destruct level_value as [v|] eqn:hv; constructor; lia.
-Qed.
-
-Lemma level_value_MapsTo {l k} {m : model} :
-  LevelMap.MapsTo l k m -> level_value m l = k.
-Proof.
-  unfold level_value.
- move=> mapto; rewrite (LevelMap.find_1 mapto) //.
-Qed.
-
-Lemma level_value_MapsTo' {l k} {m : model} :
-  level_value m l = Some k -> LevelMap.MapsTo l (Some k) m.
-Proof.
-  unfold level_value. destruct LevelMap.find eqn:hfind => //.
-  eapply LevelMap.find_2 in hfind. now intros [= ->].
-Qed.
-
-Lemma strict_update_ext m cl m' : strict_update m cl m' -> m ⩽ m'.
-Proof.
-  destruct cl as [prems [concl k]].
-  unfold strict_update.
-  intros [v [hm ha heq]].
-  intros x k' hin. setoid_rewrite heq.
-  setoid_rewrite LevelMapFact.F.add_mapsto_iff.
-  destruct (Level.eq_dec concl x). subst.
-  move: ha; rewrite /level_value_above.
-  eapply level_value_MapsTo in hin. rewrite hin.
-  intros hlt'.
-  exists (Some (k + v)).
-  split. left. split; reflexivity.
-  move/negbTE: hlt'.
-  destruct k' => //.
-  elim: Z.leb_spec => //. intros; constructor; lia. constructor.
-  exists k'. split => //. right; eauto. reflexivity.
-Qed.
-
-Lemma strictly_updates_ext cls w m m' : strictly_updates cls w m m' -> m ⩽ m'.
-Proof.
-  induction 1.
-  now eapply strict_update_ext in H0.
-  now transitivity m'.
-Qed.
-
-Lemma check_model_le {cls acc acc'} :
-  check_model cls acc = Some acc' -> acc.2 ⩽ acc'.2.
-Proof.
-  destruct acc as [w m], acc' as [w' m'].
-  move/check_model_spec => [w'' [su ->]].
-  cbn. now eapply strictly_updates_ext.
-Qed.
-
-Lemma level_value_update_model m l k :
-  level_value (update_model m l k) l = Some k.
-Proof.
-  unfold level_value, update_model.
-  cbn -[LevelMap.find LevelMap.add].
-  rewrite LevelMapFact.F.add_o.
-  destruct LevelMap.OT.eq_dec => //.
-  exfalso. now apply n.
-Qed.
-
-Lemma model_map_outside_weaken {W W'} {m m' : model} :
-  model_map_outside W m m' ->
-  W ⊂_lset W' ->
-  model_map_outside W' m m'.
-Proof.
-  intros hm sub x hin k.
-  apply hm. intros hin'. apply sub in hin'. now apply hin.
-Qed.
-
-Lemma is_model_union {cls cls' m} :
-  is_model cls m -> is_model cls' m -> is_model (Clauses.union cls cls') m.
-Proof.
-  rewrite /is_model. rewrite /is_true -!ClausesFact.for_all_iff.
-  now move=> ism ism' x /Clauses.union_spec [].
-Qed.
-
-Lemma model_le_values {m m' : model} x : m ⩽ m' -> level_value m x ≤ level_value m' x.
-Proof.
-  intros lem. specialize (lem x).
-  unfold level_value.
-  destruct LevelMap.find eqn:hl => //.
-  - apply LevelMap.find_2 in hl. specialize (lem _ hl) as [k' [mapsto leq]].
-    now rewrite (LevelMap.find_1 mapsto).
-  - constructor.
-Qed.
-
-Infix "⊂_clset" := Clauses.Subset (at level 70).
-
-Lemma max_gain_in cl cls :
-  Clauses.In cl cls ->
-  (Z.to_nat (gain cl) <= max_gain cls)%nat.
-Proof.
-  intros hin.
-  unfold max_gain. revert cl hin.
-  eapply ClausesProp.fold_rec.
-  - intros s' ise hin. firstorder eauto.
-  - intros x a s' s'' xs nxs' hadd IH cl' hin'.
-    eapply hadd in hin' as [].
-    * subst x. lia.
-    * specialize (IH _ H). lia.
-Qed.
-
-Definition max_gain_subset (cls cls' : Clauses.t) :
-  cls ⊂_clset cls' ->
-  (max_gain cls <= max_gain cls')%nat.
-Proof.
-  unfold max_gain at 1.
-  revert cls'.
-  eapply ClausesProp.fold_rec.
-  - intros s' ise sub. lia.
-  - intros x a s' s'' xs nxs' hadd IH cls'' hs.
-    specialize (IH cls''). forward IH. transitivity s'' => //.
-    intros ??. now apply hadd.
-    assert (incls'' : Clauses.In x cls'').
-    { now apply hs, hadd. }
-    apply max_gain_in in incls''. lia.
-Qed.
-
-Lemma max_clause_premise_spec cl cls :
-  Clauses.In cl cls ->
-  (premise_max (premise cl) <= max_clause_premise cls)%Z.
-Proof.
-  intros hin.
-  unfold max_clause_premise. revert cl hin.
-  eapply ClausesProp.fold_rec.
-  - intros s' ise hin. firstorder eauto.
-  - intros x a s' s'' xs nxs' hadd IH cl' hin'.
-    eapply hadd in hin' as [].
-    * subst x. lia.
-    * specialize (IH _ H). lia.
-Qed.
-
-Notation cls_diff cls W := (Clauses.diff (cls ↓ W) (cls ⇂ W)) (only parsing).
-
-(*
-  Equations? extend_model {W cls} (m : valid_model W (cls ⇂ W))
-    (r : result W (Clauses.diff (cls ↓ W) (cls ⇂ W)))
-    : result W (cls ↓ W) :=
-    extend_model _ Loop := Loop;
-    extend_model m (Model w m' sub) :=
-      Model w {| model_model := m'.(model_model) |} _.
-  Proof.
-    - apply LevelSet.subset_spec in sub. now apply clauses_conclusions_clauses_with_concl in H.
-    - eapply sub. now eapply m.(model_clauses_conclusions).
-    - apply m.
-    - eapply LevelSet.subset_spec. eapply LevelSet.subset_spec in sub.
-      now transitivity V.
-  Qed.
-
-  *)
-
-Lemma not_mem l s : ~~ LevelSet.mem l s <-> ~ LevelSet.In l s.
-Proof.
-  split. apply contraNnot. apply LevelSet.mem_spec.
-  eapply contra_notN; tea. now move/LevelSet.mem_spec.
-Qed.
 
 Lemma v_minus_w_bound_irrel {W} m m' :
   model_map_outside W m m' ->
@@ -1061,329 +70,7 @@ Proof.
   - now apply out.
 Qed.
 
-Definition max_premise_value (m : model) (l : nonEmptyLevelExprSet) : option Z :=
-  let (hd, tl) := NonEmptySetFacts.to_nonempty_list l in
-  fold_left (fun min atom => option_map2 Z.max (levelexpr_value m atom) min) tl (levelexpr_value m hd).
-
-Definition non_W_atoms W (l : LevelExprSet.t) :=
-  LevelExprSet.filter (fun lk => ~~ LevelSet.mem lk.1 W) l.
-
-Lemma non_W_atoms_spec W l : forall x, LevelExprSet.In x (non_W_atoms W l) <-> LevelExprSet.In x l /\ ~ LevelSet.In x.1 W.
-Proof.
-  intros x. now rewrite /non_W_atoms LevelExprSet.filter_spec -not_mem.
-Qed.
-
-Lemma non_W_atoms_subset W l : non_W_atoms W l ⊂_leset l.
-Proof. intros x. now rewrite /non_W_atoms LevelExprSet.filter_spec. Qed.
-
-Lemma levelexprset_levels_spec_aux l (e : LevelExprSet.t) acc :
-  LevelSet.In l (LevelExprSet.fold (fun le : LevelExprSet.elt => LevelSet.add (level le)) e acc) <->
-  (exists k, LevelExprSet.In (l, k) e) \/ LevelSet.In l acc.
-Proof.
-  eapply LevelExprSetProp.fold_rec.
-  - intros.
-    intuition auto. destruct H1 as [k hin]. lesets.
-  - intros x a s' s'' hin nin hadd ih.
-    rewrite LevelSet.add_spec.
-    split.
-    * intros [->|].
-      left. exists x.2. red in H. subst.
-      apply hadd. cbn. left. now destruct x.
-      apply ih in H.
-      intuition auto.
-      left. destruct H0 as [k Hk]. exists k. apply hadd. now right.
-    * intros [[k ins'']|inacc].
-      eapply hadd in ins''. destruct ins''; subst.
-      + now left.
-      + right. apply ih. now left; exists k.
-      + right. intuition auto.
-Qed.
-
-Lemma levelexprset_levels_spec l (e : LevelExprSet.t) :
-  LevelSet.In l (levels e) <-> exists k, LevelExprSet.In (l, k) e.
-Proof.
-  rewrite levelexprset_levels_spec_aux. intuition auto. lsets.
-Qed.
-
-Lemma levels_exprs_non_W_atoms {W prem} :
-  LevelSet.Equal (levels (non_W_atoms W prem)) (LevelSet.diff (levels prem) W).
-Proof.
-  intros e. unfold non_W_atoms.
-  rewrite levelexprset_levels_spec LevelSet.diff_spec levelexprset_levels_spec.
-  firstorder eauto.
-  rewrite LevelExprSet.filter_spec in H. now exists x.
-  rewrite LevelExprSet.filter_spec in H. destruct H.
-  rewrite LevelSetFact.not_mem_iff.
-  destruct LevelSet.mem => //.
-  exists x.
-  rewrite LevelExprSet.filter_spec. split => //.
-  rewrite LevelSetFact.not_mem_iff in H0. now rewrite H0.
-Qed.
-
-Lemma levelexprset_empty_levels x : LevelExprSet.Empty x <-> LevelSet.Empty (levels x).
-Proof.
-  split.
-  - intros he.
-    intros l hin.
-    eapply levelexprset_levels_spec in hin as [k hin]. lesets.
-  - intros emp l hin. eapply emp. eapply (levelexprset_levels_spec l.1). exists l.2.
-    now destruct l.
-Qed.
-
-Lemma non_W_atoms_ne W cl cls :
-  Clauses.In cl (cls_diff cls W) ->
-  LevelExprSet.is_empty (non_W_atoms W (premise cl)) = false.
-Proof.
-  intros x.
-  apply Clauses.diff_spec in x as [clw clr].
-  eapply in_clauses_with_concl in clw as [clw incls].
-  apply/negbTE.
-  apply/(contra_notN _ clr).
-  intros he. rewrite in_restrict_clauses. split => //.
-  epose proof (@levels_exprs_non_W_atoms W (premise cl)).
-  eapply LevelExprSetFact.is_empty_2 in he.
-  intros x hin. eapply levelexprset_empty_levels in he. rewrite H in he.
-  specialize (he x). rewrite LevelSet.diff_spec in he. intuition auto.
-  rewrite -LevelSet.mem_spec in H1 |- *. destruct LevelSet.mem; intuition auto.
-Qed.
-
 Local Open Scope Z_scope.
-
-Section MoreNonEmpty.
-
-  Import LevelExprSet.
-  Lemma In_elements {x} {s : LevelExprSet.t} : In x s <-> List.In x (elements s).
-  Proof.
-    split. now move/LevelExprSetFact.elements_1/InA_In_eq.
-    now move/InA_In_eq/LevelExprSetFact.elements_2.
-  Qed.
-  Import NonEmptySetFacts.
-
-  Notation min_opt := (option_map2 Z.min).
-  Lemma Zmin_opt_left x y : min_opt x y ≤Z x.
-  Proof.
-    destruct x as [x|], y as [y|]; constructor. lia.
-  Qed.
-
-  Lemma Zmin_opt_right x y : min_opt x y ≤Z y.
-  Proof.
-    destruct x as [x|], y as [y|]; constructor. lia.
-  Qed.
-
-  Lemma min_opt_spec x y z : min_opt x y = z -> (z = y \/ z = x).
-  Proof.
-    destruct x as [x|], y as [y|], z as [z|]; cbn; intuition auto.
-    - noconf H. pose proof (Zmin_irreducible x y). destruct H; intuition (f_equal; auto).
-    - noconf H.
-  Qed.
-
-  Lemma min_premise_spec_aux (m : model) s k :
-    min_premise m s = k ->
-    (forall x, LevelExprSet.In x s -> (k ≤Z min_atom_value m x)) /\
-    (exists x, LevelExprSet.In x s /\ k = min_atom_value m x).
-  Proof.
-    unfold min_premise.
-    move: (to_nonempty_list_spec s).
-    destruct (to_nonempty_list s). intros heq.
-    setoid_rewrite In_elements. rewrite -heq. clear s heq.
-    intros <-.
-    induction l.
-    - cbn.
-      split. intros x [->|] => //. reflexivity.
-      now exists p; split => //.
-    - destruct IHl as [ha hex].
-      split.
-      * intros x hin.
-        eapply (in_elt_inv x a [p]) in hin as [<-|inih].
-        { cbn. rewrite fold_left_comm.
-          { intros x' y z. rewrite assoc. now rewrite (comm (min_atom_value m y)) -assoc. }
-          apply Zmin_opt_left. }
-      specialize (ha _ inih).
-      cbn. rewrite fold_left_comm.
-      { intros x' y z. rewrite assoc. now rewrite (comm (min_atom_value m y)) -assoc. }
-      etransitivity; [apply Zmin_opt_right|assumption].
-      * destruct hex as [minval [inmin ih]].
-        cbn. rewrite fold_left_comm.
-        { intros x' y z. rewrite assoc. now rewrite (comm (min_atom_value m y)) -assoc. }
-        rewrite ih.
-        destruct (min_opt_spec (min_atom_value m a) (min_atom_value m minval) _ eq_refl).
-        { rewrite H. exists minval. cbn in inmin. split; [intuition|reflexivity]. }
-        { rewrite H. exists a. cbn in inmin. split; [intuition|reflexivity]. }
-  Qed.
-
-  Lemma min_premise_spec (m : model) (s : nonEmptyLevelExprSet) :
-    (forall x, LevelExprSet.In x s -> min_premise m s ≤Z min_atom_value m x) /\
-    (exists x, LevelExprSet.In x s /\ min_premise m s = min_atom_value m x).
-  Proof.
-    now apply min_premise_spec_aux.
-  Qed.
-
-  Lemma min_premise_subset (m : model) (s s' : nonEmptyLevelExprSet) :
-    LevelExprSet.Subset s s' ->
-    min_premise m s' ≤Z min_premise m s.
-  Proof.
-    intros sub.
-    have [has [mins [ins eqs]]] := min_premise_spec m s.
-    have [has' [mins' [ins' eqs']]] := min_premise_spec m s'.
-    specialize (sub _ ins). specialize (has' _ sub).
-    now rewrite eqs.
-  Qed.
-
-  Lemma premise_min_spec_aux s k :
-    premise_min s = k ->
-    (forall x, LevelExprSet.In x s -> (k <= x.2)%Z) /\
-    (exists x, LevelExprSet.In x s /\ k = x.2).
-  Proof.
-    unfold premise_min.
-    move: (to_nonempty_list_spec s).
-    destruct (to_nonempty_list s). intros heq.
-    setoid_rewrite In_elements. rewrite -heq. clear s heq.
-    intros <-.
-    induction l.
-    - cbn.
-      split. intros x [->|] => //. reflexivity.
-      now exists p; split => //.
-    - destruct IHl as [ha hex].
-      split; intros.
-      eapply (in_elt_inv x a [p]) in H as [<-|inih].
-      cbn. rewrite fold_left_comm. lia. lia.
-      specialize (ha _ inih).
-      cbn. rewrite fold_left_comm. lia. lia.
-      destruct hex as [minval [inmin ih]].
-      cbn. rewrite fold_left_comm. lia.
-      destruct (Z.leb_spec a.2 minval.2).
-      exists a. split; [intuition|]. rewrite -ih in H. lia.
-      exists minval.
-      cbn in inmin; split; [intuition auto|]. lia.
-  Qed.
-
-  Lemma premise_min_spec (s : nonEmptyLevelExprSet) :
-    (forall x, LevelExprSet.In x s -> premise_min s <= x.2) /\
-    (exists x, LevelExprSet.In x s /\ premise_min s = x.2).
-  Proof.
-    now apply premise_min_spec_aux.
-  Qed.
-
-  Lemma premise_max_spec_aux s k :
-    premise_max s = k ->
-    (forall x, LevelExprSet.In x s -> x.2 <= k) /\
-    (exists x, LevelExprSet.In x s /\ k = x.2).
-  Proof.
-    unfold premise_max.
-    move: (to_nonempty_list_spec s).
-    destruct (to_nonempty_list s). intros heq.
-    setoid_rewrite In_elements. rewrite -heq. clear s heq.
-    intros <-.
-    induction l.
-    - cbn.
-      split. intros x [->|] => //. reflexivity.
-      now exists p; split => //.
-    - destruct IHl as [ha hex].
-      split; intros.
-      eapply (in_elt_inv x a [p]) in H as [<-|inih].
-      cbn. rewrite fold_left_comm. lia. lia.
-      specialize (ha _ inih).
-      cbn. rewrite fold_left_comm. lia. lia.
-      destruct hex as [maxval [inmin ih]].
-      cbn. rewrite fold_left_comm. lia.
-      destruct (Z.leb_spec a.2 maxval.2).
-      exists maxval. cbn in inmin; split; [intuition auto|].
-      lia.
-      exists a. split; [intuition|]. rewrite -ih in H. cbn in inmin.
-      lia.
-  Qed.
-
-  Lemma premise_max_spec (s : nonEmptyLevelExprSet) :
-    (forall x, LevelExprSet.In x s -> x.2 <= premise_max s) /\
-    (exists x, LevelExprSet.In x s /\ premise_max s = x.2).
-  Proof.
-    now apply premise_max_spec_aux.
-  Qed.
-
-  Lemma premise_min_subset (s s' : nonEmptyLevelExprSet) :
-    LevelExprSet.Subset s s' ->
-    (premise_min s' <= premise_min s).
-  Proof.
-    intros sub.
-    have [has [mins [ins eqs]]] := premise_min_spec s.
-    have [has' [mins' [ins' eqs']]] := premise_min_spec s'.
-    specialize (sub _ ins). specialize (has' _ sub).
-    lia.
-  Qed.
-
-  Lemma fold_comm_assoc_nat x y z : option_map2 Nat.max x (option_map2 Nat.max y z) =
-    option_map2 Nat.max y (option_map2 Nat.max x z).
-  Proof.
-    now rewrite (assoc (f := option_map2 Nat.max)) (comm (f := option_map2 Nat.max) x y) -assoc.
-  Qed.
-
-  Lemma fold_comm_assoc x y z : option_map2 Z.max x (option_map2 Z.max y z) =
-    option_map2 Z.max y (option_map2 Z.max x z).
-  Proof.
-    now rewrite (assoc (f := option_map2 Z.max)) (comm (f := option_map2 Z.max) x y) -assoc.
-  Qed.
-
-  Notation max_opt := (option_map2 Z.max).
-
-  Lemma max_opt_spec x y z : max_opt x y = Some z -> exists x' y', x = Some x' /\ y = Some y' /\ z = Z.max x' y'.
-  Proof.
-    destruct x as [x|], y as [y|]; cbn; intuition eauto; try noconf H.
-    exists x, y. auto.
-  Qed.
-
-  Lemma max_premise_value_spec_aux (m : model) s k :
-    max_premise_value m s = Some k ->
-    (forall x, LevelExprSet.In x s -> exists k', levelexpr_value m x = Some k' /\ Some k' ≤ Some k) /\
-    (exists x, LevelExprSet.In x s /\ Some k = levelexpr_value m x).
-  Proof.
-    unfold max_premise_value.
-    move: (to_nonempty_list_spec s).
-    destruct (to_nonempty_list s). intros heq.
-    setoid_rewrite In_elements. rewrite -heq. clear s heq.
-    induction l in k |- *.
-    - cbn.
-      intros eq.
-      split. intros x [->|] => //. exists k. split => //. reflexivity.
-      now exists p; split => //.
-    - cbn. rewrite fold_left_comm. intros; apply fold_comm_assoc.
-      intros heq. apply max_opt_spec in heq as [y' [z' [eqa [eqf ->]]]].
-      specialize (IHl _ eqf). destruct IHl as [ha hex].
-      split; intros.
-      eapply (in_elt_inv x a [p]) in H as [<-|inih].
-      { exists y'; intuition eauto. constructor; lia. }
-      { specialize (ha _ inih) as [k' []]. exists k'; intuition eauto. constructor. depelim H0; lia. }
-      destruct hex as [maxval [inmax ih]].
-      cbn.
-      destruct (Z.leb_spec z' y').
-      exists a. split; [intuition|]. rewrite eqa. f_equal. lia.
-      exists maxval. cbn in inmax; split; [intuition auto|]. rewrite -ih. f_equal; lia.
-  Qed.
-
-  Lemma max_premise_value_spec (m : model) (s : nonEmptyLevelExprSet) k :
-    max_premise_value m s = Some k ->
-    (forall x, LevelExprSet.In x s -> exists k', levelexpr_value m x = Some k' /\ Some k' ≤ Some k) /\
-    (exists x, LevelExprSet.In x s /\ Some k = levelexpr_value m x).
-  Proof.
-    apply (max_premise_value_spec_aux m s).
-  Qed.
-End MoreNonEmpty.
-
-Lemma min_premise_pos_spec {m prem k} :
-  min_premise m prem = Some k ->
-  forall x, LevelExprSet.In x prem -> Some (x.2 + k)%Z ≤Z levelexpr_value m x.
-Proof.
-  pose proof (min_premise_spec m prem) as [amin [exmin [inminpre eqminpre]]].
-  intros hprem x hin.
-  specialize (amin _ hin).
-  unfold min_atom_value in amin.
-  destruct x as [l k']; cbn in *. unfold levelexpr_value; cbn.
-  destruct (level_value m l) eqn:he.
-  - depelim amin.
-    rewrite H0 in hprem. depelim hprem. constructor. lia.
-    constructor.
-    rewrite H in hprem; depelim hprem.
-  - depelim amin. rewrite H in hprem. depelim hprem.
-Qed.
 
 Lemma v_minus_w_bound_spec W m :
   forall x, ~ LevelSet.In x W -> level_value m x ≤ Some (v_minus_w_bound W m).
@@ -1421,73 +108,6 @@ Proof.
     destruct LevelMap.find => hf; depelim hf; constructor; lia.
 Qed.
 
-Lemma clauses_levels_restrict_clauses cls W :
-  clauses_levels (cls ⇂ W) ⊂_lset W.
-Proof.
-  intros x [cl []] % clauses_levels_spec.
-  eapply in_restrict_clauses in H as [hconc hprem incl].
-  eapply clause_levels_spec in H0 as []. apply hprem, H. now subst x.
-Qed.
-
-Lemma clauses_conclusions_levels cls :
-  clauses_conclusions cls ⊂_lset clauses_levels cls.
-Proof.
-  intros x.
-  rewrite clauses_conclusions_spec clauses_levels_spec.
-  setoid_rewrite clause_levels_spec.
-  firstorder auto.
-Qed.
-
-Record model_extension W m m' :=
-  { model_ext_le : m ⩽ m';
-    model_ext_same_domain : model_same_domain m m';
-    model_ext_same_outside : model_map_outside W m m' }.
-
-#[local] Instance model_ext_reflexive W : Reflexive (model_extension W).
-Proof.
-  intros m; split; reflexivity.
-Qed.
-
-#[local] Instance model_ext_transitive W : Transitive (model_extension W).
-Proof.
-  intros m m' m'' h h'; split; (etransitivity; [apply h|apply h']).
-Qed.
-
-Lemma model_extension_weaken W W' m m' :
-  W ⊂_lset W' ->
-  model_extension W m m' ->
-  model_extension W' m m'.
-Proof.
-  intros leW []; split => //.
-  eapply model_map_outside_weaken; tea.
-Qed.
-
-Lemma model_ext_trans_weaken W W' m m' m'' :
-  W ⊂_lset W' ->
-  model_extension W m m' ->
-  model_extension W' m' m'' ->
-  model_extension W' m m''.
-Proof.
-  intros leW mext mext'. eapply model_extension_weaken in mext; tea.
-  now etransitivity; tea.
-Qed.
-
-Definition model_of V (m : model) :=
-  forall k, LevelSet.In k V -> LevelMap.In k m.
-
-Definition defined_model_of V (m : model) :=
-  forall l, LevelSet.In l V -> exists k, LevelMap.MapsTo l (Some k) m.
-
-Definition only_model_of V (m : model) :=
-  forall k, LevelSet.In k V <-> exists x, LevelMap.MapsTo k x m.
-
-Lemma only_model_of_model_of {V m} : only_model_of V m -> model_of V m.
-Proof.
-  intros om l. move/om. intros [k hm]; now exists k.
-Qed.
-
-Coercion only_model_of_model_of : only_model_of >-> model_of.
-
 Definition check_model_invariants cls w m w' m' (modified : bool) :=
   if modified then
     [/\ w ⊂_lset w',
@@ -1501,62 +121,7 @@ Definition check_model_invariants cls w m w' m' (modified : bool) :=
           model_of w' m']
   else (w, m) = (w', m') /\ model_of w m.
 
-Lemma nEmpty_exists ls : ~ (LevelSet.Empty ls) -> exists l, LevelSet.In l ls.
-Proof.
-  intros ne.
-  destruct (LevelSet.choose ls) eqn:isempty. exists e.
-  now apply LevelSet.choose_spec1 in isempty.
-  now apply LevelSet.choose_spec2 in isempty.
-Qed.
-
-Lemma inLevelSet (ls : LevelSet.t) l : LevelSet.In l ls \/ ~ (LevelSet.In l ls).
-Proof.
-  lsets.
-Qed.
-
-Lemma level_value_above_MapsTo m l k : level_value_above m l k -> exists k', LevelMap.MapsTo l k' m /\ (Some k ≤ k').
-Proof.
-  unfold level_value_above.
-  destruct level_value eqn:hl => //.
-  move/Z.leb_le => hle; exists (Some z).
-  eapply level_value_MapsTo' in hl. split => //. now constructor.
-Qed.
-
-Lemma level_value_above_MapsTo' m l k k' : LevelMap.MapsTo l k' m -> (Some k ≤ k') -> level_value_above m l k.
-Proof.
-  unfold level_value_above.
-  intros H; apply LevelMap.find_1 in H. rewrite /level_value H.
-  destruct k'. intros h; depelim h.
-  now apply Z.leb_le. intros h; depelim h.
-Qed.
-
-Lemma level_value_add m l k : level_value (LevelMap.add l (Some k) m) l = Some k.
-Proof.
-  rewrite /level_value LevelMapFact.F.add_eq_o //.
-Qed.
-
-#[local] Instance clauses_conclusions_proper : Proper (Clauses.Equal ==> LevelSet.Equal) clauses_conclusions.
-Proof.
-  intros cls cls' eq x.
-  rewrite !clauses_conclusions_spec. now setoid_rewrite eq.
-Qed.
-
-#[local] Instance And3P_proper : Proper (iff ==> iff ==> iff ==> iff) ssrbool.and3.
-Proof.
-  repeat intro. split; intros []; split; intuition auto.
-Qed.
-
-#[local] Instance And4P_proper : Proper (iff ==> iff ==> iff ==> iff ==> iff) ssrbool.and4.
-Proof.
-  repeat intro. split; intros []; split; intuition auto.
-Qed.
-
-#[local] Instance And5P_proper : Proper (iff ==> iff ==> iff ==> iff ==> iff ==> iff) ssrbool.and5.
-Proof.
-  repeat intro. split; intros []; split; intuition auto.
-Qed.
-
-#[local] Instance check_model_invariants_proper :
+#[export] Instance check_model_invariants_proper :
   Proper (Clauses.Equal ==> eq ==> eq ==> eq ==> eq ==> eq ==> iff) check_model_invariants.
 Proof.
   intros cls cls' eqcls.
@@ -1564,65 +129,6 @@ Proof.
   unfold check_model_invariants.
   destruct y3 => //.
   now setoid_rewrite <-eqcls.
-Qed.
-
-Lemma min_atom_value_levelexpr_value m l a lv : min_atom_value m l = Some a -> levelexpr_value m l = Some lv ->
-  (a <= lv - l.2).
-Proof.
-  destruct l as [l k]; cbn. unfold levelexpr_value. cbn. destruct level_value => //.
-  intros [= <-] [= <-]. lia.
-Qed.
-
-Lemma clauses_conclusions_add cl cls :
-  clauses_conclusions (Clauses.add cl cls) =_lset
-  (LevelSet.singleton (level (concl cl)) ∪
-    clauses_conclusions cls).
-Proof.
-  intros x.
-  rewrite LevelSet.union_spec !clauses_conclusions_spec.
-  setoid_rewrite Clauses.add_spec; setoid_rewrite LevelSet.singleton_spec.
-  firstorder eauto. subst. now left.
-Qed.
-
-Definition declared_model_level (m : model) l := LevelMap.In l m.
-
-Definition update_model_same_domain {m l k} :
-  declared_model_level m l ->
-  model_same_domain m (update_model m l k).
-Proof.
-  unfold update_model, declared_model_level.
-  intros hin x.
-  rewrite LevelMapFact.F.add_in_iff. intuition auto. now subst.
-Qed.
-
-Definition update_model_outside {m w l k} :
-  model_map_outside (LevelSet.add l w) m (update_model m l k).
-Proof.
-  unfold update_model, model_map_outside.
-  intros l'. rewrite LevelSet.add_spec.
-  intros hin k'.
-  rewrite LevelMapFact.F.add_neq_mapsto_iff //.
-  intros heq. red in heq; subst l'. apply hin. now left.
-Qed.
-
-Lemma opt_lt_le_trans x y z :
-  opt_le Z.lt x y ->
-  opt_le Z.le y z ->
-  opt_le Z.lt x z.
-Proof.
-  intros [] H'; depelim H'; constructor. lia.
-Qed.
-
-Lemma model_of_update w m l k : model_of w m -> model_of (LevelSet.add l w) (update_model m l k).
-Proof.
-  rewrite /model_of => hint l'. rewrite LevelSet.add_spec.
-  intros [->|hadd].
-  - exists (Some k). now apply LevelMap.add_1.
-  - specialize (hint _ hadd). unfold update_model.
-    destruct hint as [x hx].
-    destruct (eqb_spec l l'). subst.
-    now exists (Some k); apply LevelMap.add_1.
-    now exists x; eapply LevelMap.add_2.
 Qed.
 
 Definition levelset_m_eq : list Level.t × model -> list Level.t × model -> Prop :=
@@ -1634,121 +140,6 @@ Proof.
   intros x y []; split => //.
   intros x y z [] []; split => //.
   all:etransitivity; tea.
-Qed.
-
-(* Definition optm := optm *)
-
-(* #[local] Instance update_value_proper : Proper (LevelMap.Equal ==> eq ==> opt ) update_value. *)
-
-#[local] Instance check_clause_model_proper : Proper (eq ==> levelset_m_eq ==> levelset_m_eq) check_clause_model.
-Proof.
-  intros x y eq [] [] []; cbn in *; subst.
-  unfold levelset_m_eq.
-  replace (update_value m y) with (update_value m0 y). split => //; destruct update_value => //.
-  unfold update_value. setoid_rewrite H0.
-Abort.
-
-Instance model_map_outside_proper : Proper (LevelSet.Equal ==> LevelMap.Equal ==> LevelMap.Equal ==> iff) model_map_outside.
-Proof.
-  intros ? ? eqcl ? ? eqm ? ? eqs.
-  unfold model_map_outside.
-  setoid_rewrite eqcl. now setoid_rewrite eqm; setoid_rewrite eqs.
-Qed.
-
-#[local] Instance proper_levelexprset_levels : Proper (LevelExprSet.Equal ==> LevelSet.Equal)
-  levels.
-Proof.
-  intros s s' eq l.
-  rewrite !levelexprset_levels_spec.
-  firstorder eauto.
-Qed.
-
-Lemma min_premise_spec' {m prems z} : min_premise m prems = Some z ->
-  (forall l k, LevelExprSet.In (l, k) prems ->
-  exists v, level_value m l = Some v /\ z <= (v - k))%Z.
-Proof.
-  intros hmin.
-  have [hall hhmin'] := min_premise_spec m prems.
-  intros l k hin; specialize (hall _ hin). rewrite hmin in hall.
-  depelim hall. destruct level_value => //. noconf H0. exists z0. split => //.
-Qed.
-
-Lemma nonEmptyLevelExprSet_elim {P : nonEmptyLevelExprSet -> Prop} :
-  (forall le, P (singleton le)) ->
-  (forall le prems, P prems -> ~ LevelExprSet.In le prems -> P (add le prems)) ->
-  forall prems, P prems.
-Proof.
-  intros hs ha.
-  intros [].
-  revert t_set0 t_ne0.
-  apply: LevelExprSetProp.set_induction; eauto.
-  - move=> s /LevelExprSetFact.is_empty_1 he ne; exfalso => //. congruence.
-  - intros s s' IH x nin hadd hne.
-    destruct (LevelExprSet.is_empty s) eqn:hem in |- .
-    eapply LevelExprSetFact.is_empty_2 in hem.
-      assert (singleton x = {| t_set := s'; t_ne := hne |}) as <- => //.
-      unfold singleton. apply eq_univ_equal. cbn.
-      intros a. specialize (hadd a). rewrite hadd.
-      rewrite LevelExprSet.singleton_spec. firstorder. subst. reflexivity.
-      specialize (IH hem).
-      specialize (ha x _ IH).
-      assert (LevelExprSet.Equal (add x {| t_set := s; t_ne := hem|}) {| t_set := s'; t_ne := hne |}).
-      2:{ apply eq_univ_equal in H. now rewrite -H. }
-      intros x'. specialize (hadd x'). rewrite LevelExprSet.add_spec.
-      cbn. firstorder. subst x'. now left.
-Qed.
-
-Lemma min_premise_pres {m m'} prems : m ⩽ m' -> min_premise m prems ≤Z min_premise m' prems.
-Proof.
-  intros ext.
-  destruct (min_premise m prems) eqn:hmin.
-  have leq := min_premise_spec' hmin. 2:constructor.
-  have [leq' e'] := min_premise_spec m' prems.
-  destruct (min_premise_spec m prems) as [_ [minz [inminz eqminz]]].
-  rewrite hmin in eqminz.
-  rewrite eqminz. destruct e' as [min' []]. rewrite H0.
-  transitivity (min_atom_value m min').
-  2:{ unfold min_atom_value. destruct min'.
-    unfold level_value. destruct (LevelMap.find t m) eqn:hfind. 2:constructor.
-    apply LevelMap.find_2 in hfind. apply ext in hfind as [k' [hfind hle]].
-    apply LevelMap.find_1 in hfind. rewrite hfind. depelim hle; constructor. lia.
-    }
-  destruct min'. specialize (leq _ _ H) as [? []].
-  unfold min_atom_value at 2. rewrite H1. rewrite -eqminz. constructor. lia.
-Qed.
-
-Lemma level_value_above_mon m m' l k : m ⩽ m' -> level_value_above m l k -> level_value_above m' l k.
-Proof.
-  intros ext; move/level_value_above_MapsTo => [v [hm hleq]].
-  eapply ext in hm. destruct hm as [v' [hm' leq']].
-  eapply level_value_above_MapsTo'; tea. transitivity v => //.
-Qed.
-
-Lemma model_of_subset V V' m :
-  model_of V m -> V' ⊂_lset V -> model_of V' m.
-Proof.
-  intros ih hv k. specialize (ih k).
-  now move/hv.
-Qed.
-
-Instance only_model_of_proper : Proper (LevelSet.Equal ==> LevelMap.Equal ==> iff) only_model_of.
-Proof.
-  intros ? ? eq ? ? eq'.
-  rewrite /only_model_of. now setoid_rewrite eq; setoid_rewrite eq'.
-Qed.
-
-Lemma only_model_of_eq V V' m :
-  only_model_of V m -> V' =_lset V -> only_model_of V' m.
-Proof.
-  intros ih hv k. now rewrite hv.
-Qed.
-
-Lemma clauses_conclusions_subset {cls cls'} :
-  Clauses.Subset cls cls' ->
-  clauses_conclusions cls ⊂_lset clauses_conclusions cls'.
-Proof.
-  intros hsub x. rewrite !clauses_conclusions_spec.
-  intuition eauto. destruct H as [cl []]; exists cl; split; try clsets; auto.
 Qed.
 
 Lemma check_model_ext {cls w init_model m w' m'} :
@@ -1879,7 +270,7 @@ Proof.
     now apply in_clauses_with_concl in hin as [hin _]. }
   depelim hlt.
   enough (k + z <= (v_minus_w_bound W m) + k - premise_min preml)%Z. lia.
-  assert (min_premise m prem ≤Z min_premise m preml)%Z.
+  assert (min_premise m prem ≤ min_premise m preml)%Z.
   { eapply min_premise_subset. eapply non_W_atoms_subset. }
   rewrite hmin in H1. depelim H1.
   transitivity (k + y)%Z. lia.
@@ -1977,7 +368,7 @@ Lemma add_expr_add_expr n n' lk : add_expr n (add_expr n' lk) = add_expr (n + n'
 Proof. destruct lk; unfold add_expr. f_equal; lia. Qed.
 Definition add_prems n s := map (add_expr n) s.
 
-Lemma In_add_prems k (prems : nonEmptyLevelExprSet):
+Lemma In_add_prems k (prems : premises):
   forall le, LevelExprSet.In le (add_prems k prems) <->
     exists le', LevelExprSet.In le' prems /\ le = add_expr k le'.
 Proof.
@@ -2080,7 +471,7 @@ Variant in_pred_closure cls : clause -> Prop :=
 Derive Signature for in_pred_closure.
 
 Inductive entails (cls : clauses) : clause -> Prop :=
-| clause_in (prems : nonEmptyLevelExprSet) (concl : LevelExpr.t) :
+| clause_in (prems : premises) (concl : LevelExpr.t) :
   LevelExprSet.In concl prems -> entails cls (prems, concl)
 | clause_cut prems' concl' prems concl :
   in_pred_closure cls (prems', concl') ->
@@ -2088,20 +479,20 @@ Inductive entails (cls : clauses) : clause -> Prop :=
   LevelExprSet.Subset prems' prems ->
   entails cls (prems, concl).
 
-Definition entails_all cls (prems concls : nonEmptyLevelExprSet) :=
+Definition entails_all cls (prems concls : premises) :=
   LevelExprSet.For_all (fun le => entails cls (prems, le)) concls.
 
 Notation " cls ⊢ prems → concl " := (entails cls (prems, concl)) (at level 20).
 Notation " cls ⊢a prems → concl " := (entails_all cls prems concl) (at level 20).
 
-Lemma in_pred_closure_equal cls (prems prems' : nonEmptyLevelExprSet) concl :
+Lemma in_pred_closure_equal cls (prems prems' : premises) concl :
   LevelExprSet.Equal prems prems' ->
   in_pred_closure cls (prems, concl) -> in_pred_closure cls (prems', concl).
 Proof.
   intros eq. apply NonEmptySetFacts.eq_univ_equal in eq. now subst prems.
 Qed.
 
-Lemma entails_equal cls (prems prems' : nonEmptyLevelExprSet) concl :
+Lemma entails_equal cls (prems prems' : premises) concl :
   LevelExprSet.Equal prems prems' ->
   entails cls (prems, concl) -> entails cls (prems', concl).
 Proof.
@@ -2235,7 +626,7 @@ Proof.
     eapply (in_pred_closure_shift _ H).
 Qed.
 
-Lemma entails_subset cls (prems prems' : nonEmptyLevelExprSet) concl : LevelExprSet.Subset prems prems' ->
+Lemma entails_subset cls (prems prems' : premises) concl : LevelExprSet.Subset prems prems' ->
   entails cls (prems, concl) ->
   entails cls (prems', concl).
 Proof.
@@ -2284,7 +675,7 @@ Lemma entails_weak_union {cls prem concl concl'} :
 Proof.
   intros hyp.
   move: concl'.
-  apply: nonEmptyLevelExprSet_elim.
+  apply: premises_elim.
   - intros le. rewrite univ_union_comm univ_union_add_singleton.
     now apply entails_weak.
   - intros le prems ih.
@@ -2332,7 +723,7 @@ Proof.
   now apply he in hin.
 Qed.
 
-Lemma entails_all_subset {cls} {prems prems' prems'' : nonEmptyLevelExprSet} :
+Lemma entails_all_subset {cls} {prems prems' prems'' : premises} :
   prems'' ⊂_leset prems' ->
   cls ⊢a prems → prems' ->
   cls ⊢a prems → prems''.
@@ -2389,7 +780,7 @@ Lemma entails_cumul_one {cls prems prems' concl} :
   entails cls (prems, concl).
 Proof.
   revert prems' prems concl.
-  apply: nonEmptyLevelExprSet_elim.
+  apply: premises_elim.
   - intros. specialize (H le). forward H by now apply LevelExprSet.singleton_spec.
     cbn in H.
     eapply entails_add; tea.
@@ -2481,7 +872,7 @@ Proof.
 Qed.
 
 
-Lemma entails_all_shift {cls : clauses} {prems concl : univ} (n : Z) :
+Lemma entails_all_shift {cls : clauses} {prems concl : premises} (n : Z) :
   cls ⊢a prems → concl ->
   cls ⊢a add_prems n prems → add_prems n concl.
 Proof.
@@ -2524,10 +915,10 @@ Proof.
 Qed.
 
 
-Definition to_clauses (prems : nonEmptyLevelExprSet) (concl : nonEmptyLevelExprSet) : clauses :=
+Definition to_clauses (prems : premises) (concl : premises) : clauses :=
   LevelExprSet.fold (fun lk cls => Clauses.add (prems, lk) cls) concl Clauses.empty.
 
-Definition is_loop (cls : clauses) (t : nonEmptyLevelExprSet) :=
+Definition is_loop (cls : clauses) (t : premises) :=
   let cls' := to_clauses t (succ_prems t) in
   Clauses.For_all (fun cl' => entails cls cl') cls'.
 
@@ -2552,7 +943,7 @@ Proof.
 Qed.
 
 #[program]
-Definition of_level_set (ls : LevelSet.t) n (hne : ~ LevelSet.Empty ls) : nonEmptyLevelExprSet :=
+Definition of_level_set (ls : LevelSet.t) n (hne : ~ LevelSet.Empty ls) : premises :=
   {| t_set := levelexprset_of_levels ls n |}.
 Next Obligation.
   apply not_Empty_is_empty => he. apply hne.
@@ -2584,7 +975,7 @@ Proof.
 Qed.
 
 Inductive result (V U : LevelSet.t) (cls : clauses) (m : model) :=
-  | Loop (v : univ) (islooping : loop_on_univ cls v)
+  | Loop (v : premises) (islooping : loop_on_univ cls v)
   | Model (w : LevelSet.t) (m : valid_model V w m cls) (prf : U ⊂_lset w).
 Arguments Loop {V U cls m}.
 Arguments Model {V U cls m}.
@@ -3134,7 +1525,7 @@ Section InnerLoop.
     assert (ne : LevelExprSet.is_empty prem' = false).
     { now eapply (non_W_atoms_ne W (prem, (l, k)) cls). }
     set (preml := {| t_set := prem'; t_ne := ne |}).
-    assert (min_premise m prem ≤Z min_premise m preml).
+    assert (min_premise m prem ≤ min_premise m preml).
     { eapply min_premise_subset. eapply non_W_atoms_subset. }
     (* min_i (f(x_i)-k_i) <= max_i(f(x_i)) - min(k_i) *)
     pose proof (min_premise_spec m preml) as [amin [exmin [inminpre eqminpre]]].
@@ -3143,7 +1534,7 @@ Section InnerLoop.
     pose proof (max_premise_value_spec m preml _ eqmaxp) as [amax [exmax [inmaxpre eqmaxpre]]].
     rewrite -eqmaxp in eqmaxpre.
     pose proof (premise_min_spec preml) as [apmin [expmin [inpminpre eqpminpre]]].
-    assert (min_premise m preml ≤Z Some (maxpreml - premise_min preml))%Z.
+    assert (min_premise m preml ≤ Some (maxpreml - premise_min preml))%Z.
     { rewrite eqminpre in H1.
       specialize (amax _ inminpre). destruct amax as [k' [lk' hk']].
       depelim hk'.
@@ -3518,7 +1909,7 @@ Section InnerLoop.
   Qed.
 
 
-  Lemma min_premise_preserved {m m'} {prems : univ} :
+  Lemma min_premise_preserved {m m'} {prems : premises} :
     (forall x, LevelSet.In x (levels prems) -> level_value m x = level_value m' x) ->
     min_premise m prems = min_premise m' prems.
   Proof.
@@ -3583,7 +1974,7 @@ Section InnerLoop.
    apply LevelMapFact.F.not_find_in_iff in he'. firstorder.
   Qed.
 
-  Lemma min_premise_restrict m W (prems : univ) v :
+  Lemma min_premise_restrict m W (prems : premises) v :
     (forall l k, LevelExprSet.In (l, k) prems -> LevelSet.In l W) ->
     min_premise (restrict_model W m) prems = Some v ->
     min_premise m prems = Some v.
@@ -4563,7 +2954,7 @@ Proof.
 Qed.
 
 #[program]
-Definition of_level_map (m : LevelMap.t (option Z)) (hne : defined_map m) : nonEmptyLevelExprSet :=
+Definition of_level_map (m : LevelMap.t (option Z)) (hne : defined_map m) : premises :=
   {| t_set := LevelMap.fold (fun l k acc =>
     if k is (Some k') return _ then LevelExprSet.add (l, k') acc else acc) m LevelExprSet.empty |}.
 Next Obligation. apply not_Empty_is_empty.
@@ -4635,7 +3026,7 @@ Proof.
 Qed.
 
 
-Definition premise_values (prems : univ) m :=
+Definition premise_values (prems : premises) m :=
   NonEmptySetFacts.map (fun '(l, k) => (l, option_get 0 (level_value m l))) prems.
 
 Lemma premise_values_spec prems m :
@@ -4648,10 +3039,10 @@ Proof.
   exists z. split => //. exists(l, x); split => //. now rewrite -H0.
 Qed.
 
-Definition hyps_map (hyps : univ) m :=
+Definition hyps_map (hyps : premises) m :=
   (forall (l : Level.t) k, LevelExprSet.In (l, k) hyps <-> LevelMap.MapsTo l (Some k) m).
 
-Lemma model_hyps_entails cls m hyps (prems : univ) concl :
+Lemma model_hyps_entails cls m hyps (prems : premises) concl :
   Clauses.In (prems, concl) cls ->
   (forall l k, LevelExprSet.In (l,k) prems -> exists z, Some z ≤ level_value m l) ->
   hyps_map hyps m ->
@@ -4667,7 +3058,7 @@ Proof.
   now eapply level_value_MapsTo'.
 Qed.
 
-Lemma entails_succ cls (u v : univ) :
+Lemma entails_succ cls (u v : premises) :
   (forall l k, LevelExprSet.In (l, k) v -> exists k', LevelExprSet.In (l, k') u /\ k <= k') ->
   cls ⊢a u → v.
 Proof.
@@ -4678,7 +3069,7 @@ Proof.
   constructor. rewrite Z2Nat.id. lia. assumption.
 Qed.
 
-Lemma hyps_entails (hyps : univ) m cls :
+Lemma hyps_entails (hyps : premises) m cls :
   hyps_map hyps m ->
   forall prems conclk, Clauses.In (prems, conclk) cls ->
   forall v, min_premise m prems = Some v ->
@@ -5193,14 +3584,14 @@ Proof.
     now constructor.
 Qed.
 
-Lemma univ_non_empty (u : univ) : ~ LevelSet.Empty (levels u).
+Lemma univ_non_empty (u : premises) : ~ LevelSet.Empty (levels u).
 Proof. intros he. have := t_ne u. move/not_Empty_is_empty.
   intros he'. apply he'. intros [l k] hin. red in he. specialize (he l). apply he.
   rewrite levelexprset_levels_spec. now exists k.
 Qed.
 
 (*
-Lemma loop_max cls (u : univ) :
+Lemma loop_max cls (u : premises) :
   cls ⊢a of_level_set (levels u) (premise_max u) (univ_non_empty u) → u.
 Proof.
   intros [l k] hin.
@@ -5254,11 +3645,11 @@ Definition max_opt_of {A} (max : A -> A -> A) (x : option A) (y : option A) : op
   | _, _ => y
   end.
 
-Definition max_premise_of l (u : univ) : option Z :=
+Definition max_premise_of l (u : premises) : option Z :=
   LevelExprSet.fold (fun '(l', k) acc => if eqb l l' then
     max_opt_of Z.max (Some k) acc else acc) u None.
 
-Lemma max_premise_of_spec l k (u : univ) : LevelExprSet.In (l, k) u -> Some k ≤ max_premise_of l u.
+Lemma max_premise_of_spec l k (u : premises) : LevelExprSet.In (l, k) u -> Some k ≤ max_premise_of l u.
 Proof.
   rewrite /max_premise_of.
   eapply LevelExprSetProp.fold_rec.
@@ -5372,7 +3763,7 @@ Definition valuation_of_result {V cls} (m : infer_result V cls) :=
 Definition to_string_expr (e : LevelExpr.t) : string :=
   let '(l, n) := e in Level.to_string l ^ (if n is Z0 then "" else "+" ^ string_of_Z n).
 
-Definition print_premise (l : nonEmptyLevelExprSet) : string :=
+Definition print_premise (l : premises) : string :=
   let (e, exprs) := NonEmptySetFacts.to_nonempty_list l in
   to_string_expr e ^
   match exprs with
@@ -5552,7 +3943,7 @@ Proof.
   rewrite heq in hp. depelim hp. now exists y.
 Qed.
 
-Lemma interp_prems_ge v (prems : nonEmptyLevelExprSet) :
+Lemma interp_prems_ge v (prems : premises) :
   forall prem, LevelExprSet.In prem prems ->
   interp_expr v prem <= interp_prems v prems.
 Proof.
@@ -5823,7 +4214,7 @@ Proof.
     rewrite (IHl a). congruence. lia.
 Qed.
 
-Lemma interp_prems_add V le (u : univ) :
+Lemma interp_prems_add V le (u : premises) :
   interp_prems V (add le u) = Z.max (interp_expr V le) (interp_prems V u).
 Proof.
   rewrite 2!interp_prems_elements.
@@ -5835,13 +4226,13 @@ Proof.
   destruct to_nonempty_list. rewrite -he //=.
 Qed.
 
-Lemma interp_prems_eq (P : univ -> Z -> Prop) V :
+Lemma interp_prems_eq (P : premises -> Z -> Prop) V :
   (forall le, P (singleton le) (interp_expr V le)) ->
   (forall le u k, P u k -> ~ LevelExprSet.In le u -> P (add le u) (Z.max (interp_expr V le) k)) ->
   forall u, P u (interp_prems V u).
 Proof.
   intros hs hadd.
-  eapply nonEmptyLevelExprSet_elim.
+  eapply premises_elim.
   - intros le. rewrite interp_prems_singleton. apply hs.
   - intros le prems ih hnin.
     rewrite interp_prems_add. now apply hadd.
@@ -5888,7 +4279,7 @@ Proof.
     cbn. lia.
 Qed.
 
-Lemma interp_prems_in {V le} {u : univ} : LevelExprSet.In le u -> interp_prems V u >= interp_expr V le.
+Lemma interp_prems_in {V le} {u : premises} : LevelExprSet.In le u -> interp_prems V u >= interp_expr V le.
 Proof.
   revert u.
   refine (interp_prems_eq (fun u z => LevelExprSet.In le u -> z >= interp_expr V le) V _ _).
@@ -5898,12 +4289,12 @@ Proof.
     specialize (hz hin). lia.
 Qed.
 
-Lemma clauses_sem_subset {u u' : univ} : u ⊂_leset u' ->
+Lemma clauses_sem_subset {u u' : premises} : u ⊂_leset u' ->
   forall V, interp_prems V u' >= interp_prems V u.
 Proof.
   intros hsub V.
   revert u u' hsub.
-  refine (interp_prems_eq (fun u z => forall u' : univ, u ⊂_leset u' -> interp_prems V u' >= z) V _ _).
+  refine (interp_prems_eq (fun u z => forall u' : premises, u ⊂_leset u' -> interp_prems V u' >= z) V _ _).
   - intros le u' hsing.
     specialize (hsing le). forward hsing by now apply LevelExprSet.singleton_spec.
     now apply interp_prems_in.
@@ -6262,7 +4653,7 @@ Proof.
   exists k. now eapply LevelExprSet.singleton_spec.
 Qed.
 
-Lemma max_premise_of_spec2 l k (u : univ) : LevelExprSet.In (l, k) u ->
+Lemma max_premise_of_spec2 l k (u : premises) : LevelExprSet.In (l, k) u ->
   exists k', LevelExprSet.In (l, k') u /\ max_premise_of l u = Some k'.
 Proof.
   remember (max_premise_of l u) as mp. symmetry in Heqmp.
@@ -6271,7 +4662,7 @@ Proof.
   destruct H as [nein ->]. elim nein. now exists k.
 Qed.
 
-Lemma max_premise_of_spec_in l (u : univ) : LevelSet.In l (levels u) ->
+Lemma max_premise_of_spec_in l (u : premises) : LevelSet.In l (levels u) ->
   exists k, max_premise_of l u = Some k /\ LevelExprSet.In (l, k) u.
 Proof.
   intros hexi.
@@ -6382,7 +4773,7 @@ Proof.
 Qed.
 
 Variant check_result {cls} :=
-  | IsLooping (v : univ) (islooping : loop_on_univ cls v)
+  | IsLooping (v : premises) (islooping : loop_on_univ cls v)
   | Invalid
   | Valid.
 Arguments check_result : clear implicits.
@@ -6467,7 +4858,7 @@ Qed.
 Definition invalid_entailment cls cl :=
   forall V, clauses_sem V cls -> clause_sem V cl -> False.
 
-Definition infers_univ (m : model) (u : univ) :=
+Definition infers_univ (m : model) (u : premises) :=
   exists z, min_premise m u = Some z /\ (0 <= z)%Z.
 
 Definition infers_expr (m : model) (le : LevelExpr.t) :=
@@ -6561,7 +4952,7 @@ Qed.
 Local Notation fn := (fold_left (option_map2 Z.min)).
 
 Lemma fold_left_impl n l :
-  (forall x, In x (n :: l) -> fn l n ≤Z x) /\
+  (forall x, In x (n :: l) -> fn l n ≤ x) /\
   (exists x, In x (n :: l) /\ fn l n = x).
 Proof.
   induction l in n |- *.
@@ -6651,19 +5042,19 @@ Proof.
   now rewrite option_map2_comm.
 Qed.
 
-Lemma min_premise_elim m (P : univ -> option Z -> Prop):
+Lemma min_premise_elim m (P : premises -> option Z -> Prop):
   (forall le, P (singleton le) (min_atom_value m le)) ->
   (forall prems acc le, P prems acc -> ~ LevelExprSet.In le prems -> P (add le prems) (option_map2 Z.min (min_atom_value m le) acc)) ->
   forall prems, P prems (min_premise m prems).
 Proof.
   intros hs hadd.
-  eapply nonEmptyLevelExprSet_elim.
+  eapply premises_elim.
   - intros le. rewrite /min_premise.
     rewrite singleton_to_nonempty_list. cbn. apply hs.
   - intros le prems hp. now rewrite min_premise_add.
 Qed.
 
-Lemma min_premise_add_down {m} {prems : univ} {l k} :
+Lemma min_premise_add_down {m} {prems : premises} {l k} :
   LevelExprSet.In (l, k + 1) prems ->
   forall z, min_premise m prems = Some z ->
        min_premise m (add (l, k) prems) = Some z.
@@ -6914,7 +5305,7 @@ add_max l k m with level_value m l :=
       | false => LevelMap.add l k m }
   | None => LevelMap.add l k m }.
 
-Lemma nleq k k' : ~ k ≤Z Some k' -> exists z, k = Some z /\ k' < z.
+Lemma nleq k k' : ~ k ≤ Some k' -> exists z, k = Some z /\ k' < z.
 Proof.
   destruct k.
   - exists z. split => //. eapply Znot_ge_lt => hl; apply H. constructor. lia.
@@ -7368,7 +5759,7 @@ Module CorrectModel.
     (hincl : only_model_of V init)
     (hs : clauses_levels cls ⊂_lset V)
     (cls' : clauses)
-    (hs' : clauses_levels cls' ⊂_lset V) : (t V (Clauses.union cls cls')) + univ :=
+    (hs' : clauses_levels cls' ⊂_lset V) : (t V (Clauses.union cls cls')) + premises :=
   infer_extension_correct m hincl hs cls' hs' with infer_extension m hincl hs cls' :=
     | Loop u _ => inr u
     | Model w m' _ =>
@@ -7392,7 +5783,7 @@ Module CorrectModel.
     - apply m'.
   Qed.
 
-  Equations? infer_extension_valid {V cls} (m : t V cls) cls' : option (t V (Clauses.union cls cls') + univ) :=
+  Equations? infer_extension_valid {V cls} (m : t V cls) cls' : option (t V (Clauses.union cls cls') + premises) :=
   infer_extension_valid m cls' with inspect (LevelSet.subset (clauses_levels cls') V) :=
     | exist false heq => None
     | exist true heq := Some (infer_extension_correct (model_valid m) _ _ cls' _).
@@ -7460,7 +5851,7 @@ Module Abstract.
       * apply (todo "cannot activate more clauses").
   Qed.
 
-  Equations enforce_clauses (m : t) (cls : Clauses.t) : option (t + univ) :=
+  Equations enforce_clauses (m : t) (cls : Clauses.t) : option (t + premises) :=
   enforce_clauses m cls with infer_extension_valid m.(model) cls :=
     | None => None
     | Some (inl m') => Some (inl {| model := m' |})
@@ -7471,12 +5862,11 @@ End LoopCheckingImpl.
 
 Module LoopChecking (LS : LevelSets).
   Module Impl := LoopCheckingImpl(LS).
-  Import Impl.Clauses.
-  Import Impl.Clauses.FLS.
+  Import Impl.Model.
 
   Definition model := Impl.Abstract.t.
 
-  Notation univ := LevelExprSet.nonEmptyLevelExprSet.
+  Notation univ := LS.LevelExprSet.nonEmptyLevelExprSet.
 
   Inductive constraint_type := UnivEq | UnivLe.
   Notation constraint := (univ * constraint_type * univ).
