common/theories/LoopChecking/Model.v
@@ -1,0 +1,999 @@
+(* Distributed under the terms of the MIT license. *)
+From Stdlib Require Import ssreflect ssrbool ZArith.
+From Stdlib Require Import Program RelationClasses Morphisms.
+From Stdlib Require Import Orders OrderedTypeAlt OrderedTypeEx MSetList MSetInterface MSetAVL MSetFacts FMapInterface MSetProperties MSetDecide.
+From MetaRocq.Utils Require Import utils.
+
+From MetaRocq.Common Require Universes.
+From MetaRocq.Common Require Import Common Interfaces HornClauses.
+From Equations Require Import Equations.
+Set Equations Transparent.
+
+Module Model (LS : LevelSets).
+  Module Export Clauses := Clauses(LS).
+
+  Definition model := LevelMap.t (option Z).
+  Definition equal_model (m m' : model) := LevelMap.Equal m m'.
+
+  Local Open Scope Z_scope.
+
+  Definition level_value (m : model) (level : Level.t) : option Z :=
+    match LevelMap.find level m with
+    | Some v => v
+    | None => None
+    end.
+
+  Lemma level_value_MapsTo {l k} {m : model} :
+    LevelMap.MapsTo l k m -> level_value m l = k.
+  Proof.
+    unfold level_value.
+  move=> mapto; rewrite (LevelMap.find_1 mapto) //.
+  Qed.
+
+  Lemma level_value_MapsTo' {l k} {m : model} :
+    level_value m l = Some k -> LevelMap.MapsTo l (Some k) m.
+  Proof.
+    unfold level_value. destruct LevelMap.find eqn:hfind => //.
+    eapply LevelMap.find_2 in hfind. now intros [= ->].
+  Qed.
+
+  Definition levelexpr_value (m : model) (atom : LevelExpr.t) :=
+    level_value m (level atom).
+
+  Extraction Inline levelexpr_value.
+
+  Definition min_atom_value (m : model) (atom : LevelExpr.t) : option Z :=
+    let '(l, k) := atom in
+    match level_value m l with
+    | None => None
+    | Some val => Some (val - k)%Z
+    end.
+
+  Definition min_premise (m : model) (l : premises) : option Z :=
+    let (hd, tl) := NonEmptySetFacts.to_nonempty_list l in
+    fold_left (fun min atom => option_map2 Z.min (min_atom_value m atom) min) tl (min_atom_value m hd).
+
+  Definition satisfiable_atom (m : model) (atom : Level.t * Z) : bool :=
+    let '(l, k) := atom in
+    match level_value m l with
+    | Some val => k <=? val
+    | None => false
+    end.
+
+  Definition satisfiable_premise (m : model) (l : premises) :=
+    LevelExprSet.for_all (satisfiable_atom m) l.
+
+  (* Definition valid_clause (m : model) (cl : clause) := *)
+    (* implb (satisfiable_premise m (premise cl)) (satisfiable_atom m (concl cl)). *)
+  Definition level_value_above m l k :=
+    match level_value m l with
+    | Some val => k <=? val
+    | None => false
+    end.
+
+  Definition valid_clause (m : model) (cl : clause) :=
+    let k0 := min_premise m (premise cl) in
+    match k0 with
+    | None => true
+    | Some k0 =>
+      let (l, k) := concl cl in
+      level_value_above m l (k + k0)
+    end.
+
+  Definition is_model (cls : clauses) (m : model) : bool :=
+    Clauses.for_all (valid_clause m) cls.
+
+  Inductive update_result :=
+    | VacuouslyTrue
+    | Holds
+    | DoesntHold (wm : LevelSet.t × model).
+
+  Definition update_model (m : model) l v : model := LevelMap.add l (Some v) m.
+
+  Definition update_value (m : model) (cl : clause) : option model :=
+    let k0 := min_premise m (premise cl) in
+    match k0 with
+    | None => None
+    | Some k0 =>
+      let (l, k) := concl cl in
+      (* Does the conclusion also hold?
+          We optimize a bit here, rather than adding k0 in a second stage,
+          we do it already while checking the clause. In the paper, a second
+          pass computes this.
+        *)
+      if level_value_above m l (k + k0) then None
+      else Some (update_model m l (k + k0))
+    end.
+
+  Definition check_clause_model cl '(modified, m) :=
+      match update_value m cl with
+    | None => (modified, m)
+    | Some m => (clause_conclusion cl :: modified, m)
+    end.
+
+  Definition check_model_aux (cls : clauses) (wm : list Level.t × model) : list Level.t × model :=
+    Clauses.fold check_clause_model cls wm.
+
+  (* If check_model = None then we have a model of all clauses,
+    othewise, we return Some (W', m') where W ⊂ W' and the model has
+    been updated for at least one atom l ∈ W'. *)
+  Definition check_model (cls : clauses) (wm : LevelSet.t × model) : option (LevelSet.t × model) :=
+    let '(modified, m) := check_model_aux cls ([], wm.2) in
+    match modified return option (LevelSet.t × model) with
+    | [] => None
+    | l => Some ((LevelSet.union (LevelSetProp.of_list l) wm.1), m)
+    end.
+
+  Infix "=m" := LevelMap.Equal (at level 50).
+
+  Definition strict_update m '(prems, (concl, k)) m' :=
+    exists v,
+    [/\ min_premise m prems = Some v, ~~ level_value_above m concl (k + v) &
+    m' =m (LevelMap.add concl (Some (k + v)) m)].
+
+  Inductive strictly_updates cls : LevelSet.t -> model -> model -> Prop :=
+  | update_one m cl m' : Clauses.In cl cls ->
+    strict_update m cl m' -> strictly_updates cls (LevelSet.singleton (clause_conclusion cl)) m m'
+  | update_trans {ls ls' m m' m''} :
+    strictly_updates cls ls m m' ->
+    strictly_updates cls ls' m' m'' ->
+    strictly_updates cls (LevelSet.union ls ls') m m''.
+
+  Lemma strictly_updates_step cls w m m' m'' :
+    strictly_updates cls w m m' ->
+    forall cl, Clauses.In cl cls -> strict_update m' cl m'' ->
+    strictly_updates cls (LevelSet.add (clause_conclusion cl) w) m m''.
+  Proof.
+    induction 1.
+    - intros.
+      replace (LevelSet.add (clause_conclusion cl0) (LevelSet.singleton (clause_conclusion cl)))
+        with (LevelSet.union (LevelSet.singleton (clause_conclusion cl)) (LevelSet.singleton (clause_conclusion cl0))).
+      eapply update_trans; eapply update_one; tea.
+      eapply LevelSet.eq_leibniz. red. lsets.
+    - intros.
+      specialize (IHstrictly_updates2 _ H1 H2).
+      replace (LevelSet.add (clause_conclusion cl) (LevelSet.union ls ls'))
+        with (LevelSet.union ls (LevelSet.add (clause_conclusion cl) ls')).
+      eapply update_trans; tea.
+      eapply LevelSet.eq_leibniz. red. lsets.
+  Qed.
+
+  Lemma strictly_updates_weaken cls w cls' :
+    Clauses.Subset cls cls' ->
+    forall m m', strictly_updates cls w m m' -> strictly_updates cls' w m m'.
+  Proof.
+    intros hcls m m'.
+    induction 1. constructor => //. now eapply hcls.
+    econstructor 2; tea.
+  Qed.
+
+  Lemma strictly_updates_W_trans cls m w m' cl m'' :
+    strictly_updates cls w m m' ->
+    strict_update m' cl m'' ->
+    strictly_updates (Clauses.add cl cls) (LevelSet.add (clause_conclusion cl) w) m m''.
+  Proof.
+    intros updW su.
+    destruct cl as [prems [concl k]].
+    eapply strictly_updates_step; tea.
+    - eapply strictly_updates_weaken; tea. clsets.
+    - rewrite Clauses.add_spec. left; reflexivity.
+  Qed.
+
+  #[export] Instance is_model_proper : Proper (Clauses.Equal ==> eq ==> eq) is_model.
+  Proof.
+    intros cl cl' eqcl x y ->. unfold is_model. now rewrite eqcl.
+  Qed.
+
+  #[export] Instance equal_model_equiv : Equivalence equal_model.
+  Proof. unfold equal_model.
+    split; try econstructor; eauto.
+    red. intros. now symmetry.
+    red; intros. now transitivity y.
+  Qed.
+
+  #[export] Instance level_value_proper : Proper (equal_model ==> eq ==> eq) level_value.
+  Proof.
+    intros x y eqm l ? <-. unfold level_value.
+    unfold equal_model in eqm.
+    destruct LevelMap.find eqn:hl.
+    - eapply LevelMap.find_2 in hl.
+      rewrite eqm in hl.
+      eapply LevelMap.find_1 in hl. now rewrite hl.
+    - eapply LevelMapFact.F.not_find_in_iff in hl.
+      rewrite eqm in hl.
+      eapply LevelMapFact.F.not_find_in_iff in hl.
+      now rewrite hl.
+  Qed.
+
+  #[export] Instance min_atom_value_proper : Proper (LevelMap.Equal ==> eq ==> eq) min_atom_value.
+  Proof.
+    intros m m' eqm ? ? ->. unfold min_atom_value.
+    destruct y => //.
+    now rewrite eqm.
+  Qed.
+
+  #[export] Instance min_premise_proper : Proper (LevelMap.Equal ==> eq ==> eq) min_premise.
+  Proof.
+    intros m m' eq ? ? ->.
+    unfold min_premise.
+    destruct to_nonempty_list.
+    now setoid_rewrite eq.
+  Qed.
+
+  #[export] Instance update_model_proper : Proper (LevelMap.Equal ==> eq ==> eq ==> LevelMap.Equal) update_model.
+  Proof.
+    intros m m' hm ? ? -> ? ? ->.
+    unfold update_model.
+    now rewrite hm.
+  Qed.
+
+  #[export] Instance level_value_above_proper : Proper (LevelMap.Equal ==> eq ==> eq ==> eq) level_value_above.
+  Proof.
+    intros m m' hm ? ? -> ? ? ->.
+    unfold level_value_above.
+    now rewrite hm.
+  Qed.
+
+  Instance clauses_elements_proper : Proper (Clauses.Equal ==> eq) Clauses.elements.
+  Proof.
+    intros cl cl' eq.
+    have sl := Clauses.elements_spec2 cl.
+    (* have nl := Clauses.elements_spec2w cl. *)
+    have sl' := Clauses.elements_spec2 cl'.
+    (* have nl' := Clauses.elements_spec2w cl'. *)
+    have heq := @SortA_equivlistA_eqlistA _ Logic.eq _ Clause.lt_.
+    do 3 forward heq by tc.
+    specialize (heq _ _ sl sl').
+    forward heq.
+    red. intros x.
+    rewrite -! ClausesProp.Dec.F.elements_iff. apply eq.
+    now apply eqlistA_eq.
+  Qed.
+
+  #[export] Instance check_model_aux_proper : Proper (Clauses.Equal ==> eq ==> eq) check_model_aux.
+  Proof.
+    intros ? ? eq ? ? ->.
+    rewrite /check_model_aux.
+    rewrite !ClausesProp.fold_spec_right.
+    now rewrite eq.
+  Qed.
+
+  #[export] Instance check_model_proper : Proper (Clauses.Equal ==> eq ==> eq) check_model.
+  Proof.
+    intros cls cls' eq.
+    intros wm wm' ->.
+    unfold check_model.
+    destruct (check_model_aux cls _) eqn:eqc.
+    destruct (check_model_aux cls' _) eqn:eqc' => //.
+    pose proof (check_model_aux_proper cls cls' eq ([], wm'.2) _ eq_refl).
+    rewrite eqc eqc' in H. noconf H.
+    destruct l => //.
+  Qed.
+
+  Instance strictly_updates_proper : Proper (Clauses.Equal ==> LevelSet.Equal ==> LevelMap.Equal ==> LevelMap.Equal ==> iff) strictly_updates.
+  Proof.
+    intros ? ? H ? ? H' ? ? H'' ? ? H'''.
+    eapply LevelSet.eq_leibniz in H'. subst y0.
+    split.
+    induction 1 in y, H, y1, H'', y2, H'''|- * ; [econstructor 1|econstructor 2]; eauto.
+    now rewrite <- H. move: H1; unfold strict_update. destruct cl as [premse []].
+    intros [v []]; exists v; split;
+    try setoid_rewrite <- H;
+    try setoid_rewrite <- H'';
+    try setoid_rewrite <- H'''; firstorder.
+    eapply IHstrictly_updates1; firstorder. firstorder.
+    induction 1 in x, H, x1, H'', x2, H'''|- * ; [econstructor 1|econstructor 2]; eauto.
+    now rewrite H. move: H1; unfold strict_update. destruct cl as [premse []].
+    intros [v []]; exists v; split;
+    try setoid_rewrite H;
+    try setoid_rewrite H'';
+    try setoid_rewrite H'''; firstorder.
+    eapply IHstrictly_updates1; firstorder. firstorder.
+  Qed.
+
+  Lemma update_value_valid {m cl} :
+    match update_value m cl with
+    | None => valid_clause m cl
+    | Some _ => ~~ valid_clause m cl
+    end.
+  Proof.
+    unfold update_value, valid_clause.
+    destruct cl as [prem [l k]]; cbn.
+    destruct min_premise => //.
+    unfold level_value_above;
+    destruct level_value => //.
+    destruct Z.leb => //.
+  Qed.
+
+  Lemma check_clause_model_spec {cl w m w' m'} :
+    check_clause_model cl (w, m) = (w', m') ->
+    (w = w' -> m = m' /\ valid_clause m cl) /\
+    (w <> w' -> w' = clause_conclusion cl :: w /\
+      strictly_updates (Clauses.singleton cl) (LevelSet.singleton (clause_conclusion cl)) m m').
+  Proof.
+    unfold check_clause_model.
+    destruct update_value eqn:upd; revgoals.
+    * intros [= <- <-]. split => //. split => //.
+      move: (@update_value_valid m cl). now rewrite upd.
+    * intros [= <- <-]. split => //.
+      + intros. eapply (f_equal (@List.length _)) in H. cbn in H; lia.
+      + intros _. split => //. constructor. clsets. unfold strict_update.
+        move: upd. unfold update_value.
+        destruct cl as [prems [concl k]]. cbn.
+        destruct min_premise => //.
+        destruct level_value_above eqn:hl => //.
+        intros [= <-].
+        exists z. split => //. rewrite hl. split => //.
+  Qed.
+
+  Lemma check_model_aux_spec {cls w m w' m'} :
+    check_model_aux cls (w, m) = (w', m') ->
+    (w = w' -> m = m' /\ is_model cls m) /\
+    (w <> w' -> exists pref, w' = pref ++ w /\ strictly_updates cls (LevelSetProp.of_list pref) m m').
+  Proof.
+    rewrite /check_model_aux /is_model.
+    revert w' m'.
+    eapply ClausesProp.fold_rec.
+    - intros s' he w' m' [= <- <-]. split => //. split => //.
+      eapply Clauses.for_all_spec. tc. intros x hin. now apply he in hin.
+    - clear. intros x [w'' m''] s' s'' inx nins' hadd ih w' m' cl.
+      specialize (ih _ _ eq_refl) as[].
+      split; intros; subst.
+      + eapply check_clause_model_spec in cl as [].
+        destruct (eqb_spec w' w'').
+        { subst w''. specialize (H eq_refl) as []. specialize (H1 eq_refl) as []. split => //. congruence.
+          eapply Clauses.for_all_spec in H3. eapply Clauses.for_all_spec. all:tc.
+          intros ? hin. eapply hadd in hin as []; subst; firstorder. }
+        forward H0 by auto. forward H2 by auto.
+        destruct H0 as [pref [-> su]].
+        destruct pref; cbn in *; try congruence.
+        destruct H2. eapply (f_equal (@List.length _)) in H0; cbn in H0. rewrite length_app in H0. lia.
+      + eapply check_clause_model_spec in cl as [].
+        destruct (eqb_spec w w'').
+        { subst w''. specialize (H eq_refl) as []. subst m''.
+          destruct (eqb_spec w w'); subst; try congruence.
+          specialize (H3 H) as []. subst w'. exists [clause_conclusion x]. split => //.
+          replace (LevelSetProp.of_list [clause_conclusion x]) with (LevelSet.singleton (clause_conclusion x)).
+          eapply ClausesProp.Add_Equal in hadd. rewrite hadd. eapply strictly_updates_weaken; tea. clsets.
+          eapply LevelSet.eq_leibniz. red. intros ?. rewrite LevelSetProp.of_list_1. firstorder. constructor.
+          rewrite LevelSet.singleton_spec in H3. firstorder. depelim H3. subst. lsets. depelim H3. }
+        specialize (H0 H4).
+        destruct (eqb_spec w'' w'); subst.
+        { specialize (H2 eq_refl) as []; subst m''.
+          destruct H0 as [pref []]. subst w'. exists pref; split => //.
+          eapply strictly_updates_weaken; tea. intros ? ?. eapply hadd. clsets. }
+        forward H3 by auto. destruct H3 as [->].
+        destruct H0 as [pref [-> su]]. eexists (clause_conclusion x :: pref); split => //.
+        replace (LevelSetProp.of_list (clause_conclusion x :: pref)) with (LevelSet.union (LevelSetProp.of_list pref) (LevelSet.singleton (clause_conclusion x))).
+        eapply (strictly_updates_weaken _ _ s'') in su; tea; try firstorder.
+        eapply (strictly_updates_weaken _ _ s'') in H3; tea; try firstorder.
+        2:{ intros ?; rewrite Clauses.singleton_spec. intros ->. now apply hadd. }
+        exact: update_trans _ su H3.
+        apply LevelSet.eq_leibniz. intros ?. cbn. lsets.
+  Qed.
+
+  Lemma check_model_spec {cls w m w' m'} :
+    check_model cls (w, m) = Some (w', m') ->
+    exists w'', strictly_updates cls w'' m m' /\ w' = LevelSet.union w w''.
+  Proof.
+    unfold check_model.
+    destruct check_model_aux eqn:cm.
+    apply check_model_aux_spec in cm as [].
+    destruct l => //. forward H0. auto with datatypes.
+    intros [= <- <-]. destruct H0 as [pref [heq su]].
+    rewrite app_nil_r in heq. subst pref.
+    exists (LevelSetProp.of_list (t :: l)). split => //.
+    eapply LevelSet.eq_leibniz. intros ?. cbn. lsets.
+  Qed.
+
+
+  Lemma strict_update_invalid m cl m' : strict_update m cl m' -> ~~ valid_clause m cl.
+  Proof.
+    destruct cl as [prems [concl k]].
+    cbn.
+    intros [v [him hna heq]].
+    rewrite /valid_clause. rewrite him //=.
+  Qed.
+
+  Lemma strictly_updates_invalid cls w m m' : strictly_updates cls w m m' -> ~~ is_model cls m.
+  Proof.
+    induction 1.
+    - eapply strict_update_invalid in H0.
+      apply/negbT. unfold is_model.
+      destruct Clauses.for_all eqn:fa => //.
+      eapply Clauses.for_all_spec in fa; tc. eapply fa in H.
+      now rewrite H in H0.
+    - auto.
+  Qed.
+
+  Lemma check_model_None {cls acc} :
+    check_model cls acc = None <-> is_model cls acc.2.
+  Proof.
+    unfold check_model.
+    destruct check_model_aux eqn:cm.
+    apply check_model_aux_spec in cm as [ne ex].
+    destruct l => //. split => // _. now specialize (ne eq_refl) as [].
+    split => //. forward ex by auto with datatypes. destruct ex as [pref [eq su]].
+    rewrite app_nil_r in eq; subst pref.
+    intros ism. eapply strictly_updates_invalid in su.
+    now rewrite ism in su.
+  Qed.
+
+  Lemma check_model_updates_spec {cls w init_model m w' m'} :
+    check_model cls (w, m) = Some (w', m') ->
+    forall cls', strictly_updates cls' w init_model m ->
+    strictly_updates (Clauses.union cls cls') w' init_model m' /\ w ⊂_lset w'.
+  Proof.
+    move/check_model_spec => [w'' [su ->]].
+    intros cls' su'. split.
+    eapply update_trans; eapply strictly_updates_weaken; tea; clsets. lsets.
+  Qed.
+
+  Lemma strictly_updates_non_empty {cls W m m'} :
+    strictly_updates cls W m m' -> ~ LevelSet.Empty W.
+  Proof.
+    induction 1.
+    - intros he. specialize (he (clause_conclusion cl)). lsets.
+    - intros he. apply IHstrictly_updates2. lsets.
+  Qed.
+
+  Lemma strictly_updates_non_empty_map {cls W m m'} :
+    strictly_updates cls W m m' -> ~ LevelMap.Empty m'.
+  Proof.
+    induction 1.
+    - intros he. specialize (he (clause_conclusion cl)).
+      destruct cl as [prems [concl k]].
+      destruct H0 as [? [? ? heq]].
+      setoid_rewrite heq in he. eapply (he (Some (k + x))); cbn.
+      rewrite LevelMapFact.F.add_mapsto_iff. firstorder.
+    - intros he. now apply IHstrictly_updates2.
+  Qed.
+
+  Lemma strictly_updates_incl {cls W m m'} :
+    strictly_updates cls W m m' -> W ⊂_lset clauses_conclusions cls.
+  Proof.
+    induction 1.
+    - intros x. rewrite clauses_conclusions_spec. firstorder. exists cl.
+      eapply LevelSet.singleton_spec in H1; red in H1; subst. split => //.
+    - lsets.
+  Qed.
+
+  Lemma check_model_subset {cls v} :
+    forall w' v', check_model cls v = Some (w', v') -> ~ LevelSet.Empty w'.
+  Proof.
+    intros w' v'.
+    move/check_model_spec => [w'' [su ->]].
+    eapply strictly_updates_non_empty in su. intros em. apply su. lsets.
+  Qed.
+
+  Definition model_same_domain (m m' : model) :=
+    forall l, LevelMap.In l m <-> LevelMap.In l m'.
+
+  #[export] Instance model_same_domain_refl : Reflexive model_same_domain.
+  Proof. intros m l. reflexivity. Qed.
+
+  #[export] Instance model_same_domain_trans : Transitive model_same_domain.
+  Proof. intros m m' m'' h h' l. rewrite (h l). apply h'. Qed.
+
+  Definition model_map_outside V (m m' : model) :=
+    forall l, ~ LevelSet.In l V ->
+      forall k, LevelMap.MapsTo l k m <-> LevelMap.MapsTo l k m'.
+
+  #[export] Instance model_map_outside_refl V : Reflexive (model_map_outside V).
+  Proof. intros m l. reflexivity. Qed.
+
+  #[export] Instance model_map_outside_trans V : Transitive (model_map_outside V).
+  Proof.
+    intros m m' m'' h h' l hnin k.
+    rewrite (h l hnin k). now apply h'.
+  Qed.
+
+  Definition model_rel R (m m' : model) :=
+    forall l k, LevelMap.MapsTo l k m -> exists k', LevelMap.MapsTo l k' m' /\ R k k'.
+
+  Infix "⩽" := (model_rel (opt_le Z.le)) (at level 70). (* \leqslant *)
+
+  #[export] Instance model_le_refl R (HR : Reflexive R) : Reflexive (model_rel R).
+  Proof. intros x l k map. exists k; split => //. Qed.
+
+  #[export] Instance model_le_trans R (HR : Transitive R) : Transitive (model_rel R).
+  Proof. intros m m' m'' mm' m'm'' l k map.
+    apply mm' in map as [k' [map ?]].
+    apply m'm'' in map as [k'' [map ?]]. exists k''. split => //.
+    now transitivity k'.
+  Qed.
+
+
+  Lemma valid_update_value {m cl} :
+    valid_clause m cl ->
+    match update_value m cl with
+    | None => true
+    | Some _ => false
+    end.
+  Proof.
+    unfold update_value, valid_clause.
+    destruct cl as [prem [l k]]; cbn.
+    destruct min_premise => //.
+    unfold level_value_above.
+    destruct level_value => //.
+    destruct Z.leb => //.
+  Qed.
+
+  Lemma update_model_monotone m l k : level_value m l ≤ Some k ->
+    m ⩽ update_model m l k.
+  Proof.
+    intros hl.
+    intros l' k' maps.
+    unfold update_model. cbn.
+    destruct (eqb_spec l l').
+    - subst l'. exists (Some k). move: hl.
+      unfold level_value.
+      rewrite (LevelMap.find_1 maps).
+      intros hle.
+      split => //. eapply LevelMap.add_1. eapply LevelMap.OT.eq_refl.
+    - exists k'. split => //. apply LevelMap.add_2 => //. reflexivity.
+  Qed.
+
+  Lemma update_model_not_above m l k : level_value_above m l k = false ->
+    m ⩽ update_model m l k.
+  Proof.
+    unfold level_value_above.
+    intros hlev.
+    apply update_model_monotone.
+    destruct level_value as [v|] eqn:hv; constructor; lia.
+  Qed.
+
+
+  Lemma level_value_not_above_spec m l k : level_value_above m l k = false -> opt_le Z.lt (level_value m l) (Some k).
+  Proof.
+    unfold level_value_above; destruct level_value => // hlt; constructor. lia.
+  Qed.
+
+  Lemma strict_update_ext m cl m' : strict_update m cl m' -> m ⩽ m'.
+  Proof.
+    destruct cl as [prems [concl k]].
+    unfold strict_update.
+    intros [v [hm ha heq]].
+    intros x k' hin. setoid_rewrite heq.
+    setoid_rewrite LevelMapFact.F.add_mapsto_iff.
+    destruct (Level.eq_dec concl x). subst.
+    move: ha; rewrite /level_value_above.
+    eapply level_value_MapsTo in hin. rewrite hin.
+    intros hlt'.
+    exists (Some (k + v)).
+    split. left. split; reflexivity.
+    move/negbTE: hlt'.
+    destruct k' => //.
+    elim: Z.leb_spec => //. intros; constructor; lia. constructor.
+    exists k'. split => //. right; eauto. reflexivity.
+  Qed.
+
+  Lemma strictly_updates_ext cls w m m' : strictly_updates cls w m m' -> m ⩽ m'.
+  Proof.
+    induction 1.
+    now eapply strict_update_ext in H0.
+    now transitivity m'.
+  Qed.
+
+  Lemma check_model_le {cls acc acc'} :
+    check_model cls acc = Some acc' -> acc.2 ⩽ acc'.2.
+  Proof.
+    destruct acc as [w m], acc' as [w' m'].
+    move/check_model_spec => [w'' [su ->]].
+    cbn. now eapply strictly_updates_ext.
+  Qed.
+
+  Lemma level_value_update_model m l k :
+    level_value (update_model m l k) l = Some k.
+  Proof.
+    unfold level_value, update_model.
+    cbn -[LevelMap.find LevelMap.add].
+    rewrite LevelMapFact.F.add_o.
+    destruct LevelMap.OT.eq_dec => //.
+    exfalso. now apply n.
+  Qed.
+
+  Lemma model_map_outside_weaken {W W'} {m m' : model} :
+    model_map_outside W m m' ->
+    W ⊂_lset W' ->
+    model_map_outside W' m m'.
+  Proof.
+    intros hm sub x hin k.
+    apply hm. intros hin'. apply sub in hin'. now apply hin.
+  Qed.
+
+  Lemma is_model_union {cls cls' m} :
+    is_model cls m -> is_model cls' m -> is_model (Clauses.union cls cls') m.
+  Proof.
+    rewrite /is_model. rewrite /is_true -!ClausesFact.for_all_iff.
+    now move=> ism ism' x /Clauses.union_spec [].
+  Qed.
+
+  Lemma model_le_values {m m' : model} x : m ⩽ m' -> level_value m x ≤ level_value m' x.
+  Proof.
+    intros lem. specialize (lem x).
+    unfold level_value.
+    destruct LevelMap.find eqn:hl => //.
+    - apply LevelMap.find_2 in hl. specialize (lem _ hl) as [k' [mapsto leq]].
+      now rewrite (LevelMap.find_1 mapsto).
+    - constructor.
+  Qed.
+
+
+  Lemma min_premise_spec_aux (m : model) s k :
+    min_premise m s = k ->
+    (forall x, LevelExprSet.In x s -> (k ≤ min_atom_value m x)) /\
+    (exists x, LevelExprSet.In x s /\ k = min_atom_value m x).
+  Proof.
+    unfold min_premise.
+    move: (to_nonempty_list_spec s).
+    destruct (to_nonempty_list s). intros heq.
+    setoid_rewrite In_elements. rewrite -heq. clear s heq.
+    intros <-.
+    induction l.
+    - cbn.
+      split. intros x [->|] => //. reflexivity.
+      now exists p; split => //.
+    - destruct IHl as [ha hex].
+      split.
+      * intros x hin.
+        eapply (in_elt_inv x a [p]) in hin as [<-|inih].
+        { cbn. rewrite fold_left_comm.
+          { intros x' y z. rewrite assoc. now rewrite (comm (min_atom_value m y)) -assoc. }
+          apply Zmin_opt_left. }
+      specialize (ha _ inih).
+      cbn. rewrite fold_left_comm.
+      { intros x' y z. rewrite assoc. now rewrite (comm (min_atom_value m y)) -assoc. }
+      etransitivity; [apply Zmin_opt_right|assumption].
+      * destruct hex as [minval [inmin ih]].
+        cbn. rewrite fold_left_comm.
+        { intros x' y z. rewrite assoc. now rewrite (comm (min_atom_value m y)) -assoc. }
+        rewrite ih.
+        destruct (min_opt_spec (min_atom_value m a) (min_atom_value m minval) _ eq_refl).
+        { rewrite H. exists minval. cbn in inmin. split; [intuition|reflexivity]. }
+        { rewrite H. exists a. cbn in inmin. split; [intuition|reflexivity]. }
+  Qed.
+
+  Lemma min_premise_spec (m : model) (s : premises) :
+    (forall x, LevelExprSet.In x s -> min_premise m s ≤ min_atom_value m x) /\
+    (exists x, LevelExprSet.In x s /\ min_premise m s = min_atom_value m x).
+  Proof.
+    now apply min_premise_spec_aux.
+  Qed.
+
+  Lemma min_premise_subset (m : model) (s s' : premises) :
+    LevelExprSet.Subset s s' ->
+    min_premise m s' ≤ min_premise m s.
+  Proof.
+    intros sub.
+    have [has [mins [ins eqs]]] := min_premise_spec m s.
+    have [has' [mins' [ins' eqs']]] := min_premise_spec m s'.
+    specialize (sub _ ins). specialize (has' _ sub).
+    now rewrite eqs.
+  Qed.
+
+  Lemma premise_min_spec_aux s k :
+    premise_min s = k ->
+    (forall x, LevelExprSet.In x s -> (k <= x.2)%Z) /\
+    (exists x, LevelExprSet.In x s /\ k = x.2).
+  Proof.
+    unfold premise_min.
+    move: (to_nonempty_list_spec s).
+    destruct (to_nonempty_list s). intros heq.
+    setoid_rewrite In_elements. rewrite -heq. clear s heq.
+    intros <-.
+    induction l.
+    - cbn.
+      split. intros x [->|] => //. reflexivity.
+      now exists p; split => //.
+    - destruct IHl as [ha hex].
+      split; intros.
+      eapply (in_elt_inv x a [p]) in H as [<-|inih].
+      cbn. rewrite fold_left_comm. lia. lia.
+      specialize (ha _ inih).
+      cbn. rewrite fold_left_comm. lia. lia.
+      destruct hex as [minval [inmin ih]].
+      cbn. rewrite fold_left_comm. lia.
+      destruct (Z.leb_spec a.2 minval.2).
+      exists a. split; [intuition|]. rewrite -ih in H. lia.
+      exists minval.
+      cbn in inmin; split; [intuition auto|]. lia.
+  Qed.
+
+  Lemma premise_min_spec (s : premises) :
+    (forall x, LevelExprSet.In x s -> premise_min s <= x.2) /\
+    (exists x, LevelExprSet.In x s /\ premise_min s = x.2).
+  Proof.
+    now apply premise_min_spec_aux.
+  Qed.
+
+  Lemma premise_max_spec_aux s k :
+    premise_max s = k ->
+    (forall x, LevelExprSet.In x s -> x.2 <= k) /\
+    (exists x, LevelExprSet.In x s /\ k = x.2).
+  Proof.
+    unfold premise_max.
+    move: (to_nonempty_list_spec s).
+    destruct (to_nonempty_list s). intros heq.
+    setoid_rewrite In_elements. rewrite -heq. clear s heq.
+    intros <-.
+    induction l.
+    - cbn.
+      split. intros x [->|] => //. reflexivity.
+      now exists p; split => //.
+    - destruct IHl as [ha hex].
+      split; intros.
+      eapply (in_elt_inv x a [p]) in H as [<-|inih].
+      cbn. rewrite fold_left_comm. lia. lia.
+      specialize (ha _ inih).
+      cbn. rewrite fold_left_comm. lia. lia.
+      destruct hex as [maxval [inmin ih]].
+      cbn. rewrite fold_left_comm. lia.
+      destruct (Z.leb_spec a.2 maxval.2).
+      exists maxval. cbn in inmin; split; [intuition auto|].
+      lia.
+      exists a. split; [intuition|]. rewrite -ih in H. cbn in inmin.
+      lia.
+  Qed.
+
+  Lemma premise_max_spec (s : premises) :
+    (forall x, LevelExprSet.In x s -> x.2 <= premise_max s) /\
+    (exists x, LevelExprSet.In x s /\ premise_max s = x.2).
+  Proof.
+    now apply premise_max_spec_aux.
+  Qed.
+
+  Lemma premise_min_subset (s s' : premises) :
+    LevelExprSet.Subset s s' ->
+    (premise_min s' <= premise_min s).
+  Proof.
+    intros sub.
+    have [has [mins [ins eqs]]] := premise_min_spec s.
+    have [has' [mins' [ins' eqs']]] := premise_min_spec s'.
+    specialize (sub _ ins). specialize (has' _ sub).
+    lia.
+  Qed.
+
+  Import LevelExprSet.
+  Import NonEmptySetFacts.
+
+  Definition max_premise_value (m : model) (l : premises) : option Z :=
+    let (hd, tl) := NonEmptySetFacts.to_nonempty_list l in
+    fold_left (fun min atom => option_map2 Z.max (levelexpr_value m atom) min) tl (levelexpr_value m hd).
+
+  Lemma max_premise_value_spec_aux (m : model) s k :
+    max_premise_value m s = Some k ->
+    (forall x, LevelExprSet.In x s -> exists k', levelexpr_value m x = Some k' /\ Some k' ≤ Some k) /\
+    (exists x, LevelExprSet.In x s /\ Some k = levelexpr_value m x).
+  Proof.
+    unfold max_premise_value.
+    move: (to_nonempty_list_spec s).
+    destruct (to_nonempty_list s). intros heq.
+    setoid_rewrite In_elements. rewrite -heq. clear s heq.
+    induction l in k |- *.
+    - cbn.
+      intros eq.
+      split. intros x [->|] => //. exists k. split => //. reflexivity.
+      now exists p; split => //.
+    - cbn. rewrite fold_left_comm. intros; apply fold_comm_assoc.
+      intros heq. apply max_opt_spec in heq as [y' [z' [eqa [eqf ->]]]].
+      specialize (IHl _ eqf). destruct IHl as [ha hex].
+      split; intros.
+      eapply (in_elt_inv x a [p]) in H as [<-|inih].
+      { exists y'; intuition eauto. constructor; lia. }
+      { specialize (ha _ inih) as [k' []]. exists k'; intuition eauto. constructor. depelim H0; lia. }
+      destruct hex as [maxval [inmax ih]].
+      cbn.
+      destruct (Z.leb_spec z' y').
+      exists a. split; [intuition|]. rewrite eqa. f_equal. lia.
+      exists maxval. cbn in inmax; split; [intuition auto|]. rewrite -ih. f_equal; lia.
+  Qed.
+
+  Lemma max_premise_value_spec (m : model) (s : premises) k :
+    max_premise_value m s = Some k ->
+    (forall x, LevelExprSet.In x s -> exists k', levelexpr_value m x = Some k' /\ Some k' ≤ Some k) /\
+    (exists x, LevelExprSet.In x s /\ Some k = levelexpr_value m x).
+  Proof.
+    apply (max_premise_value_spec_aux m s).
+  Qed.
+
+  Lemma min_premise_pos_spec {m prem k} :
+    min_premise m prem = Some k ->
+    forall x, LevelExprSet.In x prem -> Some (x.2 + k)%Z ≤ levelexpr_value m x.
+  Proof.
+    pose proof (min_premise_spec m prem) as [amin [exmin [inminpre eqminpre]]].
+    intros hprem x hin.
+    specialize (amin _ hin).
+    unfold min_atom_value in amin.
+    destruct x as [l k']; cbn in *. unfold levelexpr_value; cbn.
+    destruct (level_value m l) eqn:he.
+    - depelim amin.
+      rewrite H0 in hprem. depelim hprem. constructor. lia.
+      constructor.
+      rewrite H in hprem; depelim hprem.
+    - depelim amin. rewrite H in hprem. depelim hprem.
+  Qed.
+
+  Record model_extension W m m' :=
+    { model_ext_le : m ⩽ m';
+      model_ext_same_domain : model_same_domain m m';
+      model_ext_same_outside : model_map_outside W m m' }.
+
+  #[local] Instance model_ext_reflexive W : Reflexive (model_extension W).
+  Proof.
+    intros m; split; reflexivity.
+  Qed.
+
+  #[local] Instance model_ext_transitive W : Transitive (model_extension W).
+  Proof.
+    intros m m' m'' h h'; split; (etransitivity; [apply h|apply h']).
+  Qed.
+
+  Lemma model_extension_weaken W W' m m' :
+    W ⊂_lset W' ->
+    model_extension W m m' ->
+    model_extension W' m m'.
+  Proof.
+    intros leW []; split => //.
+    eapply model_map_outside_weaken; tea.
+  Qed.
+
+  Lemma model_ext_trans_weaken W W' m m' m'' :
+    W ⊂_lset W' ->
+    model_extension W m m' ->
+    model_extension W' m' m'' ->
+    model_extension W' m m''.
+  Proof.
+    intros leW mext mext'. eapply model_extension_weaken in mext; tea.
+    now etransitivity; tea.
+  Qed.
+
+  Definition model_of V (m : model) :=
+    forall k, LevelSet.In k V -> LevelMap.In k m.
+
+  Definition defined_model_of V (m : model) :=
+    forall l, LevelSet.In l V -> exists k, LevelMap.MapsTo l (Some k) m.
+
+  Definition only_model_of V (m : model) :=
+    forall k, LevelSet.In k V <-> exists x, LevelMap.MapsTo k x m.
+
+  Lemma only_model_of_model_of {V m} : only_model_of V m -> model_of V m.
+  Proof.
+    intros om l. move/om. intros [k hm]; now exists k.
+  Qed.
+
+  Coercion only_model_of_model_of : only_model_of >-> model_of.
+
+  Lemma level_value_above_MapsTo m l k : level_value_above m l k -> exists k', LevelMap.MapsTo l k' m /\ (Some k ≤ k').
+  Proof.
+    unfold level_value_above.
+    destruct level_value eqn:hl => //.
+    move/Z.leb_le => hle; exists (Some z).
+    eapply level_value_MapsTo' in hl. split => //. now constructor.
+  Qed.
+
+  Lemma level_value_above_MapsTo' m l k k' : LevelMap.MapsTo l k' m -> (Some k ≤ k') -> level_value_above m l k.
+  Proof.
+    unfold level_value_above.
+    intros H; apply LevelMap.find_1 in H. rewrite /level_value H.
+    destruct k'. intros h; depelim h.
+    now apply Z.leb_le. intros h; depelim h.
+  Qed.
+
+  Lemma level_value_add m l k : level_value (LevelMap.add l (Some k) m) l = Some k.
+  Proof.
+    rewrite /level_value LevelMapFact.F.add_eq_o //.
+  Qed.
+
+  Definition declared_model_level (m : model) l := LevelMap.In l m.
+
+  Definition update_model_same_domain {m l k} :
+    declared_model_level m l ->
+    model_same_domain m (update_model m l k).
+  Proof.
+    unfold update_model, declared_model_level.
+    intros hin x.
+    rewrite LevelMapFact.F.add_in_iff. intuition auto. now subst.
+  Qed.
+
+  Definition update_model_outside {m w l k} :
+    model_map_outside (LevelSet.add l w) m (update_model m l k).
+  Proof.
+    unfold update_model, model_map_outside.
+    intros l'. rewrite LevelSet.add_spec.
+    intros hin k'.
+    rewrite LevelMapFact.F.add_neq_mapsto_iff //.
+    intros heq. red in heq; subst l'. apply hin. now left.
+  Qed.
+
+  Lemma min_atom_value_levelexpr_value m l a lv : min_atom_value m l = Some a -> levelexpr_value m l = Some lv ->
+    (a <= lv - l.2).
+  Proof.
+    destruct l as [l k]; cbn. unfold levelexpr_value. cbn. destruct level_value => //.
+    intros [= <-] [= <-]. lia.
+  Qed.
+
+  Lemma model_of_update w m l k : model_of w m -> model_of (LevelSet.add l w) (update_model m l k).
+  Proof.
+    rewrite /model_of => hint l'. rewrite LevelSet.add_spec.
+    intros [->|hadd].
+    - exists (Some k). now apply LevelMap.add_1.
+    - specialize (hint _ hadd). unfold update_model.
+      destruct hint as [x hx].
+      destruct (eqb_spec l l'). subst.
+      now exists (Some k); apply LevelMap.add_1.
+      now exists x; eapply LevelMap.add_2.
+  Qed.
+
+  #[export] Instance model_map_outside_proper : Proper (LevelSet.Equal ==> LevelMap.Equal ==> LevelMap.Equal ==> iff) model_map_outside.
+  Proof.
+    intros ? ? eqcl ? ? eqm ? ? eqs.
+    unfold model_map_outside.
+    setoid_rewrite eqcl. now setoid_rewrite eqm; setoid_rewrite eqs.
+  Qed.
+
+  #[export] Instance proper_levelexprset_levels : Proper (LevelExprSet.Equal ==> LevelSet.Equal)
+    levels.
+  Proof.
+    intros s s' eq l.
+    rewrite !levelexprset_levels_spec.
+    firstorder eauto.
+  Qed.
+
+  Lemma min_premise_spec' {m prems z} : min_premise m prems = Some z ->
+    (forall l k, LevelExprSet.In (l, k) prems ->
+    exists v, level_value m l = Some v /\ z <= (v - k))%Z.
+  Proof.
+    intros hmin.
+    have [hall hhmin'] := min_premise_spec m prems.
+    intros l k hin; specialize (hall _ hin). rewrite hmin in hall.
+    depelim hall. destruct level_value => //. noconf H0. exists z0. split => //.
+  Qed.
+
+  Lemma min_premise_pres {m m'} prems : m ⩽ m' -> min_premise m prems ≤ min_premise m' prems.
+  Proof.
+    intros ext.
+    destruct (min_premise m prems) eqn:hmin.
+    have leq := min_premise_spec' hmin. 2:constructor.
+    have [leq' e'] := min_premise_spec m' prems.
+    destruct (min_premise_spec m prems) as [_ [minz [inminz eqminz]]].
+    rewrite hmin in eqminz.
+    rewrite eqminz. destruct e' as [min' []]. rewrite H0.
+    transitivity (min_atom_value m min').
+    2:{ unfold min_atom_value. destruct min'.
+      unfold level_value. destruct (LevelMap.find t0 m) eqn:hfind. 2:constructor.
+      apply LevelMap.find_2 in hfind. apply ext in hfind as [k' [hfind hle]].
+      apply LevelMap.find_1 in hfind. rewrite hfind. depelim hle; constructor. lia.
+      }
+    destruct min'. specialize (leq _ _ H) as [? []].
+    unfold min_atom_value at 2. rewrite H1. rewrite -eqminz. constructor. lia.
+  Qed.
+
+  Lemma level_value_above_mon m m' l k : m ⩽ m' -> level_value_above m l k -> level_value_above m' l k.
+  Proof.
+    intros ext; move/level_value_above_MapsTo => [v [hm hleq]].
+    eapply ext in hm. destruct hm as [v' [hm' leq']].
+    eapply level_value_above_MapsTo'; tea. transitivity v => //.
+  Qed.
+
+  Lemma model_of_subset V V' m :
+    model_of V m -> V' ⊂_lset V -> model_of V' m.
+  Proof.
+    intros ih hv k. specialize (ih k).
+    now move/hv.
+  Qed.
+
+  Instance only_model_of_proper : Proper (LevelSet.Equal ==> LevelMap.Equal ==> iff) only_model_of.
+  Proof.
+    intros ? ? eq ? ? eq'.
+    rewrite /only_model_of. now setoid_rewrite eq; setoid_rewrite eq'.
+  Qed.
+
+  Lemma only_model_of_eq V V' m :
+    only_model_of V m -> V' =_lset V -> only_model_of V' m.
+  Proof.
+    intros ih hv k. now rewrite hv.
+  Qed.
+
+
+End Model.
